cfrontend/Cexec.v
@@ -20,7 +20,7 @@ Require Import AST Values Memory Events Globalenvs Builtins Determinism.
 Require Import Csem.
 Require Import Tags.
 Require Import List. Import ListNotations.
-Require Import Cstrategy Ctypes.
+Require Import InterpreterEvents Ctypes.
 
 Local Open Scope string_scope.
 Local Open Scope list_scope.
@@ -59,10 +59,22 @@ Notation " 'check' A ; B" := (if A then B else nil)
   (at level 200, A at level 100, B at level 200)
   : list_monad_scope.
 
+(* Policy-agnostic Tactics *)
+Ltac mydestr :=
+  match goal with
+  | [ |- None = Some _ -> _ ] => let X := fresh "X" in intro X; discriminate
+  | [ |- Some _ = Some _ -> _ ] => let X := fresh "X" in intro X; inv X
+  | [ |- match ?x with Some _ => _ | None => _ end = Some _ -> _ ] => destruct x eqn:?; mydestr
+  | [ |- match ?x with true => _ | false => _ end = Some _ -> _ ] => destruct x eqn:?; mydestr
+  | [ |- match ?x with inl _ => _ | inr _ => _ end = Some _ -> _ ] => destruct x; mydestr
+  | [ |- match ?x with left _ => _ | right _ => _ end = Some _ -> _ ] => destruct x; mydestr
+  | [ |- (let (_, _) := ?x in _) = Some _ -> _ ] => destruct x; mydestr
+  | _ => idtac
+  end.
+
 Module Cexec (P:Policy).
-  Module TLib := TagLib P.
-  Import TLib.
-  Module Cstrategy := Cstrategy P.
+  Module InterpreterEvents := InterpreterEvents P.
+  Import InterpreterEvents.
   Import Cstrategy.
   Import Ctyping.
   Import Csem.
@@ -75,6 +87,7 @@ Module Cexec (P:Policy).
   Import Genv.
   Import Mem.
   Import P.
+  Import Csem.TLib.
   
   Definition is_val (a: expr) : option (atom * type) :=
     match a with
@@ -119,239 +132,6 @@ Module Cexec (P:Policy).
 
     Variable ge: gcenv.
 
-    Definition eventval_of_val (a: atom) (t: typ) : option eventval :=
-      let '(v,vt) := a in
-      match v with
-      | Vint i => check (typ_eq t AST.Tint); Some (EVint i)
-      | Vfloat f => check (typ_eq t AST.Tfloat); Some (EVfloat f)
-      | Vsingle f => check (typ_eq t AST.Tsingle); Some (EVsingle f)
-      | Vlong n =>
-          if (typ_eq t AST.Tlong) then Some (EVlong n)
-          else check (typ_eq t AST.Tptr);
-          match invert_symbol_ofs (fst ge) (Ptrofs.of_int64 n) with
-          | Some id =>
-              match find_symbol (fst ge) id with
-              | Some (inr (base, bound, pt)) =>
-                  check (public_symbol (fst ge) id);
-                  check (tag_eq_dec vt pt);
-                  Some (EVptr_global id (Ptrofs.repr ((Int64.unsigned n)-base)))
-              | _ => None
-              end
-          | None => None
-          end
-      | Vfptr b =>
-          check (typ_eq t AST.Tptr);
-          do id <- invert_symbol_block (fst ge) b;
-          match find_symbol (fst ge) id with
-          | Some (inl (b,pt)) =>
-              check (public_symbol (fst ge) b);
-              check (tag_eq_dec vt pt);
-              Some (EVptr_fun id)
-          | _ => None
-          end
-      | _ => None
-      end.
-
-    Fixpoint list_eventval_of_val (vl: list atom) (tl: list typ) : option (list eventval) :=
-      match vl, tl with
-      | nil, nil => Some nil
-      | v1::vl, t1::tl =>
-          do ev1 <- eventval_of_val v1 t1;
-          do evl <- list_eventval_of_val vl tl;
-          Some (ev1 :: evl)
-      | _, _ => None
-      end.
-
-    Definition val_of_eventval (ev: eventval) (t: typ) : option atom :=
-      match ev with
-      | EVint i => check (typ_eq t AST.Tint); Some (Vint i, def_tag)
-      | EVfloat f => check (typ_eq t AST.Tfloat); Some (Vfloat f, def_tag)
-      | EVsingle f => check (typ_eq t AST.Tsingle); Some (Vsingle f, def_tag)
-      | EVlong n => check (typ_eq t AST.Tlong); Some (Vlong n, def_tag)
-      | EVptr_global id ofs =>
-        check (Genv.public_symbol (fst ge) id);
-        check (typ_eq t AST.Tptr);
-        match Genv.find_symbol (fst ge) id with
-        | Some (inr (base,bound,pt)) =>
-          Some (Vofptrsize (base + (Ptrofs.signed ofs)), pt)
-        | _ => None
-        end
-      | EVptr_fun id =>
-        check (Genv.public_symbol (fst ge) id);
-        check (typ_eq t AST.Tptr);
-        match Genv.find_symbol (fst ge) id with
-        | Some (inl (b,pt)) =>
-          Some (Vfptr b, pt)
-        | _ => None
-        end    
-      end.
-
-    Ltac mydestr :=
-      match goal with
-      | [ |- None = Some _ -> _ ] => let X := fresh "X" in intro X; discriminate
-      | [ |- Some _ = Some _ -> _ ] => let X := fresh "X" in intro X; inv X
-      | [ |- match ?x with Some _ => _ | None => _ end = Some _ -> _ ] => destruct x eqn:?; mydestr
-      | [ |- match ?x with true => _ | false => _ end = Some _ -> _ ] => destruct x eqn:?; mydestr
-      | [ |- match ?x with inl _ => _ | inr _ => _ end = Some _ -> _ ] => destruct x; mydestr
-      | [ |- match ?x with left _ => _ | right _ => _ end = Some _ -> _ ] => destruct x; mydestr
-      | [ |- (let (_, _) := ?x in _) = Some _ -> _ ] => destruct x; mydestr
-      | _ => idtac
-      end.
-
-    Lemma eventval_of_val_sound:
-      forall v t ev, eventval_of_val v t = Some ev -> eventval_match (fst ge) ev t v.
-(*    Proof.
-      intros until ev. destruct v; destruct v; simpl; mydestr; try constructor.
-      - pose (i' := Int.unsigned i).
-        replace (Int.unsigned i) with i' by auto; replace i with (Int.repr i') by apply Int.repr_unsigned.
-        admit.
-      
-      eapply ev_match_global; eauto. replace i' with (Int.unsigned i) by auto.
-      apply invert_find_symbol_ofs in Heqo. destruct Heqo as [base [bound [pt [H1 H2]]]].
-      rewrite H1 in Heqo0. inv Heqo0. destruct H2.
-      replace (Ptrofs.unsigned (Ptrofs.of_int i)) with (Int.unsigned i) in H.
-      rewrite Ptrofs.agree32_of_int in H0.
-      auto. unfold Ptrofs.of_int. rewrite Ptrofs.unsigned_repr. auto.
-      Search (Int.max_unsigned). rewrite Ptrofs.agree32.
-      eapply Int.unsigned_range_2.
-      Qed.*)
-    Admitted.
-
-    Lemma eventval_of_val_complete:
-      forall ev t v, eventval_match (fst ge) ev t v -> eventval_of_val v t = Some ev.
-(*Proof.
-  induction 1; simpl.
-- auto.
-- auto.
-- auto.
-- auto.
-- rewrite (Genv.find_invert_symbol _ _ _ H0). simpl in H; rewrite H.
-  rewrite dec_eq_true. auto.
-  admit.*)
-    Admitted.
-
-    Lemma list_eventval_of_val_sound:
-      forall vl tl evl, list_eventval_of_val vl tl = Some evl -> eventval_list_match (fst ge) evl tl vl.
-    Proof with try discriminate.
-      induction vl; destruct tl; simpl; intros; inv H.
-      constructor.
-      destruct (eventval_of_val a t0) as [ev1|] eqn:?...
-      destruct (list_eventval_of_val vl tl) as [evl'|] eqn:?...
-      inv H1. constructor. apply eventval_of_val_sound; auto. eauto.
-    Qed.
-
-    Lemma list_eventval_of_val_complete:
-      forall evl tl vl, eventval_list_match (fst ge) evl tl vl -> list_eventval_of_val vl tl = Some evl.
-    Proof.
-      induction 1; simpl. auto.
-      rewrite (eventval_of_val_complete _ _ _ H). rewrite IHeventval_list_match. auto.
-    Qed.
-
-    Lemma val_of_eventval_sound:
-      forall ev t v, val_of_eventval ev t = Some v -> eventval_match (fst ge) ev t v.
-    Admitted.
-    (*Proof.
-  intros until v. destruct ev; simpl; mydestr; constructor; auto.
-Qed.*)
-
-    Lemma val_of_eventval_complete:
-      forall ev t v, eventval_match (fst ge) ev t v -> val_of_eventval ev t = Some v.
-    Admitted.
-    (*Proof.
-      induction 1; simpl.
-      - auto.
-      - auto.
-      - auto.
-      - auto.
-      - simpl in *. rewrite H, H0. rewrite dec_eq_true. auto.  
-      Qed.*)
-
-    (** Volatile memory accesses. *)
-    Definition do_volatile_load (w: world) (chunk: memory_chunk) (m: mem)
-               (ofs: ptrofs) : option (world * trace * atom) :=
-      if Genv.addr_is_volatile (fst ge) ofs then
-        do id <- Genv.invert_symbol_ofs (fst ge) ofs;
-        do res,w' <- nextworld_vload w chunk id ofs;
-        do vres,vt <- val_of_eventval res (type_of_chunk chunk);
-        Some(w', Event_vload chunk id ofs res :: nil,
-              (Val.load_result chunk vres, vt))
-      else
-        do v <- Mem.load chunk m (Ptrofs.unsigned ofs);
-        let lts := load_ltags chunk m (Ptrofs.unsigned ofs) in
-        Some(w, E0, v).
-
-    Definition do_volatile_store (w: world) (chunk: memory_chunk) (m: mem)
-               (ofs: ptrofs) (v: atom) (lts: list tag) : option (world * trace * mem * atom) :=
-      if Genv.addr_is_volatile (fst ge) ofs then
-        do id <- Genv.invert_symbol_ofs (fst ge) ofs;
-        do ev <- eventval_of_val (atom_map (Val.load_result chunk) v) (type_of_chunk chunk);
-        do w' <- nextworld_vstore w chunk id ofs ev;
-        Some(w', Event_vstore chunk id ofs ev :: nil, m, v)
-      else
-        do m' <- Mem.store chunk m (Ptrofs.unsigned ofs) v lts;
-        Some(w, E0, m', v).
-
-    Lemma do_volatile_load_sound:
-      forall w chunk m ofs w' t v,
-        do_volatile_load w chunk m ofs = Some(w', t, v) ->
-        volatile_load (fst ge) chunk m ofs t v /\ possible_trace w t w'.
-    Proof.
-      intros until v. unfold do_volatile_load. mydestr.
-      - split.
-        + constructor; auto. apply val_of_eventval_sound; auto.
-        + econstructor. econstructor. eauto. constructor.
-      - split.
-        + constructor; auto.
-        + constructor.
-    Qed.
-
-    Lemma do_volatile_load_complete:
-      forall w chunk m ofs w' t v,
-        volatile_load (fst ge) chunk m ofs t v -> possible_trace w t w' ->
-        do_volatile_load w chunk m ofs = Some(w', t, v).
-    Admitted.
-(*    Proof.
-      unfold do_volatile_load; intros.
-      inv H; simpl in *.
-      - rewrite H1. destruct (invert_symbol_ofs (fst ge) ofs).
-        + admit.
-        + 
-
-          rewrite (Genv.find_invert_symbol _ _ H2). inv H0. inv H8. inv H6. rewrite H9.
-    rewrite (val_of_eventval_complete _ _ _ H3). auto.
-  - rewrite H1. rewrite H2. inv H0. auto.
-  - destruct b; unfold dummy in *.
-    + simpl. rewrite H2. inv H0. auto.
-    + simpl. rewrite H2. inv H0. auto.
-    + contradiction.
-Qed.*)
-
-    Lemma do_volatile_store_sound:
-      forall w chunk m ofs v w' t m' v' lts,
-        do_volatile_store w chunk m ofs v lts = Some(w', t, m', v') ->
-        volatile_store (fst ge) chunk m ofs v lts t m' /\ possible_trace w t w' /\ v' = v.
-    Admitted.
-(*Proof.
-  intros until v'. unfold do_volatile_store. mydestr.
-  split. constructor; auto. apply Genv.invert_find_symbol; auto.
-  apply eventval_of_val_sound; auto.
-  split. econstructor. constructor; eauto. constructor. auto.
-  split. constructor; auto. split. constructor. auto.
-Qed.*)
-
-    Lemma do_volatile_store_complete:
-      forall w chunk m ofs v w' t m' lts,
-        volatile_store (fst ge) chunk m ofs v lts t m' -> possible_trace w t w' ->
-        do_volatile_store w chunk m ofs v lts = Some(w', t, m', v).
-    Admitted.
-(*Proof.
-  unfold do_volatile_store; intros. inv H; simpl in *.
-  rewrite H1. rewrite (Genv.find_invert_symbol _ _ H2).
-  rewrite (eventval_of_val_complete _ _ _ H3).
-  inv H0. inv H8. inv H6. rewrite H9. auto.
-  rewrite H1. rewrite H2. inv H0. auto.
-Qed.*)
-
 (** Accessing locations *)
 
     Definition do_deref_loc (w: world) (ty: type) (m: mem) (ofs: ptrofs) (pt:tag) (bf: bitfield) : option (world * trace * atom * list tag) :=
@@ -361,7 +141,7 @@ Qed.*)
           | By_value chunk =>
               match type_is_volatile ty with
               | false => do v <- Mem.load chunk m (Ptrofs.unsigned ofs); Some(w, E0, v, load_ltags chunk m (Ptrofs.unsigned ofs))
-              | true => option_map (fun x => (x, load_ltags chunk m (Ptrofs.unsigned ofs))) (do_volatile_load w chunk m ofs)
+              | true => option_map (fun x => (x, load_ltags chunk m (Ptrofs.unsigned ofs))) (do_volatile_load ge w chunk m ofs)
               end
           | By_reference => Some(w, E0, (Vofptrsize (Ptrofs.unsigned ofs),pt), [])
           | By_copy => Some(w, E0, (Vofptrsize (Ptrofs.unsigned ofs),pt),[])
@@ -417,7 +197,7 @@ Qed.*)
           | By_value chunk =>
               match type_is_volatile ty with
               | false => do m' <- Mem.store chunk m (Ptrofs.unsigned ofs) v lts; Some(w, E0, m', v)
-              | true => do_volatile_store w chunk m ofs v lts
+              | true => do_volatile_store ge w chunk m ofs v lts
               end
           | By_copy =>
               match v with
@@ -454,9 +234,9 @@ Qed.*)
       destruct bf.
       - destruct (access_mode ty) eqn:?; mydestr.
         + intros. exploit do_volatile_load_sound; eauto.
-          destruct (do_volatile_load w m0 m ofs) eqn:?; simpl in H; inv H. eauto.
+          destruct (do_volatile_load ge w m0 m ofs) eqn:?; simpl in H; inv H. eauto.
           intuition. eapply deref_loc_volatile; eauto.
-          destruct (do_volatile_load w m0 m ofs); simpl in H; inv H. auto.
+          destruct (do_volatile_load ge w m0 m ofs); simpl in H; inv H. auto.
         + split.
           * eapply deref_loc_value; eauto;
               (destruct Archi.ptr64;
@@ -478,7 +258,7 @@ Qed.*)
     Proof.
       unfold do_deref_loc; intros. inv H.
       - inv H0. rewrite H3; rewrite H4. rewrite H7; auto.
-      - rewrite H3; rewrite H4. apply (do_volatile_load_complete w _ _ _ w') in H7.
+      - rewrite H3; rewrite H4. apply (do_volatile_load_complete ge w _ _ _ w') in H7.
         rewrite H7. simpl. auto. apply H0.
       - inv H0. rewrite H6. auto.
       - inv H0. rewrite H6. auto.
@@ -563,8 +343,8 @@ Hypothesis do_inline_assembly_complete:
 Definition do_ef_volatile_load (chunk: memory_chunk)
        (w: world) (vargs: list val) (m: mem) : option (world * trace * atom * mem) :=
   match vargs with
-  | Vint ofs :: nil => do w',t,v <- do_volatile_load w chunk m (Ptrofs.of_int ofs); Some(w',t,v,m)
-  | Vlong ofs :: nil => do w',t,v <- do_volatile_load w chunk m (Ptrofs.of_int64 ofs); Some(w',t,v,m)
+  | Vint ofs :: nil => do w',t,v <- do_volatile_load ge w chunk m (Ptrofs.of_int ofs); Some(w',t,v,m)
+  | Vlong ofs :: nil => do w',t,v <- do_volatile_load ge w chunk m (Ptrofs.of_int64 ofs); Some(w',t,v,m)
   | _ => None
   end.
 
@@ -825,444 +605,480 @@ Inductive reduction: Type :=
 | Callred (rule: string) (fd: fundef) (args: list atom) (tyres: type) (pct': tag) (te': tenv) (m': mem)
 | Stuckred (*anaaktge enters impossible state or would have to take impossible step. 
               think like a /0 *)
-| Failstopred (msg: string) (params: list tag) (tr: trace)
+| Failstopred (rule: string) (msg: string) (params: list tag) (tr: trace)
            (* anaaktge - for tag fail stops add things here. dont add it to stuck *)
 .
 
 Section EXPRS.
 
-Variable e: env.
-Variable w: world.
+  Variable e: env.
+  Variable w: world.
 
-Fixpoint sem_cast_arguments (vtl: list (atom * type)) (tl: typelist) (m: mem) : option (list atom) :=
-  match vtl, tl with
-  | nil, Tnil => Some nil
-  | (v1,vt1,t1)::vtl, Tcons t1' tl =>
-      do v <- sem_cast v1 t1 t1' m; do vl <- sem_cast_arguments vtl tl m; Some((v,vt1)::vl)
-  | _, _ => None
-  end.
+  Fixpoint sem_cast_arguments (vtl: list (atom * type)) (tl: typelist) (m: mem) : option (list atom) :=
+    match vtl, tl with
+    | nil, Tnil => Some nil
+    | (v1,vt1,t1)::vtl, Tcons t1' tl =>
+        do v <- sem_cast v1 t1 t1' m; do vl <- sem_cast_arguments vtl tl m; Some((v,vt1)::vl)
+    | _, _ => None
+    end.
 
-(** The result of stepping an expression is a list [ll] of possible reducts.
-  Each element of [ll] is a pair of a context and the result of reducing
-  inside this context (see type [reduction] above).
-  The list [ll] is empty if the expression is fully reduced
-   (it's [Eval] for a r-value and [Eloc] of [Efloc] for a l-value).
-*)
+  (** The result of stepping an expression is a list [ll] of possible reducts.
+      Each element of [ll] is a pair of a context and the result of reducing
+      inside this context (see type [reduction] above).
+      The list [ll] is empty if the expression is fully reduced
+      (it's [Eval] for a r-value and [Eloc] of [Efloc] for a l-value).
+   *)
 
-Definition reducts (A: Type): Type := list ((expr -> A) * reduction).
+  Definition reducts (A: Type): Type := list ((expr -> A) * reduction).
 
-Definition topred (r: reduction) : reducts expr :=
-  ((fun (x: expr) => x), r) :: nil.
+  Definition topred (r: reduction) : reducts expr :=
+    ((fun (x: expr) => x), r) :: nil.
 
-Definition failred (msg : string) (params : list tag) (tr : trace) : reducts expr :=
-  ((fun (x: expr) => x), Failstopred msg params tr) :: nil.
+  Definition failred (rule : string) (msg : string) (params : list tag) (tr : trace) : reducts expr :=
+    ((fun (x: expr) => x), Failstopred rule msg params tr) :: nil.
 
-Definition stuck : reducts expr :=
-  ((fun (x: expr) => x), Stuckred) :: nil.
+  Definition stuck : reducts expr :=
+    ((fun (x: expr) => x), Stuckred) :: nil.
 
-Definition incontext {A B: Type} (ctx: A -> B) (ll: reducts A) : reducts B :=
-  map (fun z => ((fun (x: expr) => ctx(fst z x)), snd z)) ll.
+  Definition incontext {A B: Type} (ctx: A -> B) (ll: reducts A) : reducts B :=
+    map (fun z => ((fun (x: expr) => ctx(fst z x)), snd z)) ll.
+  
+  Definition incontext2 {A1 A2 B: Type}
+             (ctx1: A1 -> B) (ll1: reducts A1)
+             (ctx2: A2 -> B) (ll2: reducts A2) : reducts B :=
+    incontext ctx1 ll1 ++ incontext ctx2 ll2.
+  
+  Notation "'do' X <- A ; B" := (match A with Some X => B | _ => stuck end)
+                                  (at level 200, X name, A at level 100, B at level 200)
+      : reducts_monad_scope.
 
-Definition incontext2 {A1 A2 B: Type}
-                     (ctx1: A1 -> B) (ll1: reducts A1)
-                     (ctx2: A2 -> B) (ll2: reducts A2) : reducts B :=
-  incontext ctx1 ll1 ++ incontext ctx2 ll2.
+  Notation "'do' X , Y <- A ; B" := (match A with Some (X, Y) => B | None => stuck end)
+                                      (at level 200, X name, Y name, A at level 100, B at level 200)
+      : reducts_monad_scope.
 
-Notation "'do' X <- A ; B" := (match A with Some X => B | None => stuck end)
-  (at level 200, X name, A at level 100, B at level 200)
-  : reducts_monad_scope.
+  Notation "'do' X , Y , Z <- A ; B" := (match A with Some (X, Y, Z) => B | None => stuck end)
+                                          (at level 200, X name, Y name, Z name, A at level 100, B at level 200)
+      : reducts_monad_scope.
 
-Notation "'do' X , Y <- A ; B" := (match A with Some (X, Y) => B | None => stuck end)
-  (at level 200, X name, Y name, A at level 100, B at level 200)
-  : reducts_monad_scope.
+  Notation "'do' X , Y , Z , W <- A ; B" := (match A with Some (X, Y, Z, W) => B | None => stuck end)
+                                              (at level 200, X name, Y name, Z name, W name,
+                                                A at level 100, B at level 200)
+      : reducts_monad_scope.
 
-Notation "'do' X , Y , Z <- A ; B" := (match A with Some (X, Y, Z) => B | None => stuck end)
-  (at level 200, X name, Y name, Z name, A at level 100, B at level 200)
-  : reducts_monad_scope.
+  Notation "'dor' X , Y , Z <- A ; B" := (match A with Some (inr (X, Y, Z)) => B | _ => stuck end)
+                                           (at level 200, X name, Y name, Z name,
+                                             A at level 100, B at level 200)
+      : reducts_monad_scope.
 
-Notation "'do' X , Y , Z , W <- A ; B" := (match A with Some (X, Y, Z, W) => B | None => stuck end)
-  (at level 200, X name, Y name, Z name, W name, A at level 100, B at level 200)
-  : reducts_monad_scope.
+  Notation "'dol' X , Y <- A ; B" := (match A with Some (inl (X, Y)) => B | _ => stuck end)
+                                       (at level 200, X name, Y name, A at level 100, B at level 200)
+      : reducts_monad_scope.
 
-Notation "'dor' X , Y , Z <- A ; B" := (match A with Some (inr (X, Y, Z)) => B | _ => stuck end)
-  (at level 200, X name, Y name, Z name, A at level 100, B at level 200)
-  : reducts_monad_scope.
+  Notation " 'check' A ; B" := (if A then B else stuck)
+                                 (at level 200, A at level 100, B at level 200)
+      : reducts_monad_scope.
 
-Notation "'dol' X , Y <- A ; B" := (match A with Some (inl (X, Y)) => B | _ => stuck end)
-  (at level 200, X name, Y name, A at level 100, B at level 200)
-  : reducts_monad_scope.
+  Local Open Scope reducts_monad_scope.
 
-Notation " 'check' A ; B" := (if A then B else stuck)
-  (at level 200, A at level 100, B at level 200)
-  : reducts_monad_scope.
+  (* anaaktge - TODO does failstop give me the policy output yet? 
+     probably should do something with the str and list from PolicyFail *)
+  Notation "'at' R 'trule' X <- A ; B" :=
+    (match A with
+     | PolicySuccess X => B
+     | PolicyFail msg params => failred R msg params E0
+     end)
+      (at level 200, X name, A at level 100, B at level 200)
+      : tag_monad_scope.
 
-Local Open Scope reducts_monad_scope.
+  Notation "'at' R 'truletr' T , X <- A ; B" :=
+    (match A with
+     | PolicySuccess X => B
+     | PolicyFail msg params => failred R msg params T
+     end)
+      (at level 200, X name, A at level 100, B at level 200)
+      : tag_monad_scope.
 
-(* anaaktge - TODO does failstop give me the policy output yet? 
-    probably should do something with the str and list from PolicyFail *)
-Notation "'trule' X <- A ; B" := (match A with
-                                      | PolicySuccess X => B
-                                      | PolicyFail msg params => failred msg params E0
-                                      end)
-  (at level 200, X name, A at level 100, B at level 200)
-  : tag_monad_scope.
+  Notation "'at' R 'trule' X , Y <- A ; B" :=
+    (match A with
+     | PolicySuccess (X, Y) => B
+     | PolicyFail msg params => failred R msg params E0
+     end)
+      (at level 200, X name, Y name, A at level 100, B at level 200)
+      : tag_monad_scope.
 
-Notation "'truletr' T , X <- A ; B" := (match A with
-                                      | PolicySuccess X => B
-                                      | PolicyFail msg params => failred msg params T
-                                      end)
-  (at level 200, X name, A at level 100, B at level 200)
-  : tag_monad_scope.
+  Notation "'at' R 'truletr' T , X , Y <- A ; B" :=
+    (match A with
+     | PolicySuccess (X, Y) => B
+     | PolicyFail msg params => failred R msg params T
+     end)
+      (at level 200, X name, Y name, A at level 100, B at level 200)
+      : tag_monad_scope.
 
+  Notation "'at' R 'trule' X , Y , Z <- A ; B" :=
+    (match A with
+     | PolicySuccess (X, Y, Z) => B
+     | PolicyFail msg params => failred R msg params E0
+     end)
+      (at level 200, X name, Y name, Z name, A at level 100, B at level 200)
+      : tag_monad_scope.
 
-Notation "'trule' X , Y <- A ; B" := (match A with
-                                          | PolicySuccess (X, Y) => B
-                                          | PolicyFail msg params => failred msg params E0
-                                          end)
-  (at level 200, X name, Y name, A at level 100, B at level 200)
-  : tag_monad_scope.
+  Notation "'at' R 'truletr' T , X , Y , Z <- A ; B" :=
+    (match A with
+     | PolicySuccess (X, Y, Z) => B
+     | PolicyFail msg params => failred R msg params T
+     end)
+      (at level 200, X name, Y name, Z name, A at level 100, B at level 200)
+      : tag_monad_scope.
 
-Notation "'truletr' T , X , Y <- A ; B" := (match A with
-                                          | PolicySuccess (X, Y) => B
-                                          | PolicyFail msg params => failred msg params T
-                                          end)
-  (at level 200, X name, Y name, A at level 100, B at level 200)
-  : tag_monad_scope.
+  Notation "'at' R 'trule' X , Y , Z , W <- A ; B" :=
+    (match A with
+     | PolicySuccess (X, Y, Z, W) => B
+     | PolicyFail msg params => failred R msg params E0
+     end)
+      (at level 200, X name, Y name, Z name, W name, A at level 100, B at level 200)
+      : tag_monad_scope.
 
-Notation "'trule' X , Y , Z <- A ; B" := (match A with
-                                          | PolicySuccess (X, Y, Z) => B
-                                          | PolicyFail msg params => failred msg params E0
-                                          end)
-  (at level 200, X name, Y name, Z name, A at level 100, B at level 200)
-  : tag_monad_scope.
+  Local Open Scope tag_monad_scope.
 
-Notation "'truletr' T , X , Y , Z <- A ; B" := (match A with
-                                          | PolicySuccess (X, Y, Z) => B
-                                          | PolicyFail msg params => failred msg params T
-                                          end)
-  (at level 200, X name, Y name, Z name, A at level 100, B at level 200)
-  : tag_monad_scope.
-
-
-Notation "'trule' X , Y , Z , W <- A ; B" := (match A with
-                                              | PolicySuccess (X, Y, Z, W) => B
-                                              | PolicyFail msg params => failred msg params E0
-                                              end)
-  (at level 200, X name, Y name, Z name, W name, A at level 100, B at level 200)
-  : tag_monad_scope.
-
-Local Open Scope tag_monad_scope.
-
-Fixpoint step_expr (k: kind) (pct: tag) (a: expr) (te: tenv) (m: mem): reducts expr :=
-  match k, a with
-  | LV, Eloc l ty => []
-  | LV, Evar x ty =>
-      match e!x with
-      | Some (PUB (base, bound, pt)) =>
-          topred (Lred "red_var_local" (Eloc (Lmem (Ptrofs.repr base) pt Full) ty) te m)
-      | Some PRIV =>
-          topred (Lred "red_var_tmp" (Eloc (Ltmp x) ty) te m)
-      | None =>
-          match Genv.find_symbol (fst ge) x with
-          | Some (inr (base, bound, t)) =>
-              topred (Lred "red_var_global" (Eloc (Lmem (Ptrofs.repr base) t Full) ty) te m)
-          | Some (inl (b, t)) =>
-              topred (Lred "red_var_func" (Eloc (Lfun b t) ty) te m)
-          | None => stuck
-          end
-      end
-  | LV, Ederef r ty =>
-      match is_val r with
-      | Some (Vint ofs, t, ty') =>
-          topred (Lred "red_deref_short" (Eloc (Lmem (Ptrofs.of_int ofs) t Full) ty) te m)    
-      | Some (Vlong ofs, t, ty') =>
-          topred (Lred "red_deref_long" (Eloc (Lmem (Ptrofs.of_int64 ofs) t Full) ty) te m)
-      | Some _ =>
-          stuck
-      | None =>
-          incontext (fun x => Ederef x ty) (step_expr RV pct r te m)
-      end
-  | LV, Efield r f ty =>
-      match is_val r with
-      | Some (Vlong ofs, pt, ty') =>
-          match ty' with
-          | Tstruct id _ =>
-              do co <- (snd ge)!id;
-              match field_offset (snd ge) f (co_members co) with
-              | Error _ => stuck
-              | OK (delta, bf) =>
-                  trule pt' <- FieldT (snd ge) pct pt ty id;
-                  topred (Lred "red_field_struct" (Eloc (Lmem (Ptrofs.add
-                                                                 (Ptrofs.of_int64 ofs)
-                                                                 (Ptrofs.repr delta))
-                                                              pt' bf) ty) te m)
-              end
-          | Tunion id _ =>
-              do co <- (snd ge)!id;
-              match union_field_offset (snd ge) f (co_members co) with
-              | Error _ => stuck
-              | OK (delta, bf) =>
-                  trule pt' <- FieldT (snd ge) pct pt ty id;
-                  topred (Lred "red_field_union" (Eloc (Lmem (Ptrofs.add
-                                                                (Ptrofs.of_int64 ofs)
-                                                                (Ptrofs.repr delta))
-                                                             pt' bf) ty) te m)
-              end
-          | _ => stuck
-          end
-      | Some _ =>
-          stuck
-      | None =>
-          incontext (fun x => Efield x f ty) (step_expr RV pct r te m)
-      end
-  | RV, Eval v ty => []
-  | RV, Econst v ty =>
-      trule vt <- ConstT pct;
-      topred (Rred "red_const" pct (Eval (v,vt) ty) te m E0)
-  | RV, Evalof l ty =>
-      match is_loc l with
-      | Some (Lmem ofs pt bf, ty') =>
-          check type_eq ty ty';
-          do w',t,vvt,lts <- do_deref_loc w ty m ofs pt bf;
-          let (v,vt) := vvt in
-          truletr t, vt' <- LoadT pct pt vt lts;
-          truletr t, vt'' <- AccessT pct vt';
-          topred (Rred "red_rvalof_mem" pct (Eval (v,vt'') ty) te m t)
-      | Some (Ltmp b, ty') =>
-          check type_eq ty ty';
-          do v,vt <- te!b;
-          trule vt' <- AccessT pct vt;
-          topred (Rred "red_rvalof_tmp" pct (Eval (v,vt') ty) te m E0)
-      | Some (Lfun b pt, ty') =>
-          check type_eq ty ty';
-          topred (Rred "red_rvalof_fun" pct (Eval (Vfptr b, pt) ty) te m E0)
-      | None => incontext (fun x => Evalof x ty) (step_expr LV pct l te m)
-      end
-  | RV, Eaddrof l ty =>
-      match is_loc l with
-      | Some (Lmem ofs t bf, ty') =>
-          match bf with Full => topred (Rred "red_addrof_loc" pct
-                                             (Eval (Vofptrsize (Ptrofs.unsigned ofs), t) ty) te m E0)
-                      | Bits _ _ _ _ => stuck
-          end
-      | Some (Ltmp _, _) => stuck
-      | Some (Lfun b pt, ty') =>
-          check type_eq ty ty';
-          topred (Rred "red_addrof_floc" pct (Eval (Vfptr b, pt) ty) te m E0)
-      | None =>
-          incontext (fun x => Eaddrof x ty) (step_expr LV pct l te m)
-      end
-  | RV, Eunop op r1 ty =>
-      match is_val r1 with
-      | Some(v1, vt1, ty1) =>
-          do v <- sem_unary_operation op v1 ty1 m;
-          trule pct',vt' <- UnopT op pct vt1;
-          topred (Rred "red_unop" pct' (Eval (v,vt') ty) te m E0)
-      | None =>
-          incontext (fun x => Eunop op x ty) (step_expr RV pct r1 te m)
-      end
-  | RV, Ebinop op r1 r2 ty =>
-      match is_val r1, is_val r2 with
-      | Some(v1, vt1, ty1), Some(v2, vt2, ty2) =>
-          do v <- sem_binary_operation (snd ge) op v1 ty1 v2 ty2 m;
-          trule pct',vt' <- BinopT op pct vt1 vt2;
-          topred (Rred "red_binop" pct' (Eval (v,vt') ty) te m E0) (* TODO: control points *)
-      | _, _ =>
-         incontext2 (fun x => Ebinop op x r2 ty) (step_expr RV pct r1 te m)
-                    (fun x => Ebinop op r1 x ty) (step_expr RV pct r2 te m)
-      end
-  | RV, Ecast r1 ty =>
-      match is_val r1 with
-      | Some(v1, t1, ty1) =>
-          let tr := match ty1, ty with
-                    | _, _ => IPCastT
-                    end in          
-          do v <- sem_cast v1 ty1 ty m;
-          topred (Rred "red_cast" pct (Eval (v,t1) ty) te m E0)
-      | None =>
-          incontext (fun x => Ecast x ty) (step_expr RV pct r1 te m)
-      end
-  | RV, Eseqand r1 r2 ty =>
-      match is_val r1 with
-      | Some(v1, vt1, ty1) =>
-          do b <- bool_val v1 ty1 m;
-          trule pct' <- ExprSplitT pct vt1;
-          if b then topred (Rred "red_seqand_true" pct' (Eparen r2 type_bool ty) te m E0)
+  Fixpoint step_expr (k: kind) (pct: tag) (a: expr) (te: tenv) (m: mem): reducts expr :=
+    match k, a with
+    | LV, Eloc l ty => []
+    | LV, Evar x ty =>
+        match e!x with
+        | Some (PUB (base, bound, pt)) =>
+            topred (Lred "red_var_local" (Eloc (Lmem (Ptrofs.repr base) pt Full) ty) te m)
+        | Some PRIV =>
+            topred (Lred "red_var_tmp" (Eloc (Ltmp x) ty) te m)
+        | None =>
+            match Genv.find_symbol (fst ge) x with
+            | Some (inr (base, bound, t)) =>
+                topred (Lred "red_var_global" (Eloc (Lmem (Ptrofs.repr base) t Full) ty) te m)
+            | Some (inl (b, t)) =>
+                topred (Lred "red_var_func" (Eloc (Lfun b t) ty) te m)
+            | None => stuck
+            end
+        end
+    | LV, Ederef r ty =>
+        match is_val r with
+        | Some (Vint ofs, t, ty') =>
+            topred (Lred "red_deref_short" (Eloc (Lmem (Ptrofs.of_int ofs) t Full) ty) te m)    
+        | Some (Vlong ofs, t, ty') =>
+            topred (Lred "red_deref_long" (Eloc (Lmem (Ptrofs.of_int64 ofs) t Full) ty) te m)
+        | Some _ =>
+            stuck
+        | None =>
+            incontext (fun x => Ederef x ty) (step_expr RV pct r te m)
+        end
+    | LV, Efield r f ty =>
+        match is_val r with
+        | Some (Vlong ofs, pt, ty') =>
+            match ty' with
+            | Tstruct id _ =>
+                do co <- (snd ge)!id;
+                match field_offset (snd ge) f (co_members co) with
+                | Error _ => stuck
+                | OK (delta, bf) =>
+                    at "failred_field_struct" trule pt' <- FieldT (snd ge) pct pt ty id;
+                    topred (Lred "red_field_struct" (Eloc (Lmem (Ptrofs.add
+                                                                   (Ptrofs.of_int64 ofs)
+                                                                   (Ptrofs.repr delta))
+                                                                pt' bf) ty) te m)
+                end
+            | Tunion id _ =>
+                do co <- (snd ge)!id;
+                match union_field_offset (snd ge) f (co_members co) with
+                | Error _ => stuck
+                | OK (delta, bf) =>
+                    at "failred_field_union" trule pt' <- FieldT (snd ge) pct pt ty id;
+                    topred (Lred "red_field_union" (Eloc (Lmem (Ptrofs.add
+                                                                  (Ptrofs.of_int64 ofs)
+                                                                  (Ptrofs.repr delta))
+                                                               pt' bf) ty) te m)
+                end
+            | _ => stuck
+            end
+        | Some _ =>
+            stuck
+        | None =>
+            incontext (fun x => Efield x f ty) (step_expr RV pct r te m)
+        end
+    | RV, Eval v ty => []
+    | RV, Econst v ty =>
+        at "failred_const" trule vt <- ConstT pct;
+        topred (Rred "red_const" pct (Eval (v,vt) ty) te m E0)
+    | RV, Evalof l ty =>
+        match is_loc l with
+        | Some (Lmem ofs pt bf, ty') =>
+            check type_eq ty ty';
+            do w',t,vvt,lts <- do_deref_loc w ty m ofs pt bf;
+            let (v,vt) := vvt in
+            at "failred_rvalof_mem1" truletr t, vt' <- LoadT pct pt vt lts;
+            at "failred_rvalof_mem2" truletr t, vt'' <- AccessT pct vt';
+            topred (Rred "red_rvalof_mem" pct (Eval (v,vt'') ty) te m t)
+        | Some (Ltmp b, ty') =>
+            check type_eq ty ty';
+            do v,vt <- te!b;
+            at "failred_rvalof_tmp" trule vt' <- AccessT pct vt;
+            topred (Rred "red_rvalof_tmp" pct (Eval (v,vt') ty) te m E0)
+        | Some (Lfun b pt, ty') =>
+            check type_eq ty ty';
+            topred (Rred "red_rvalof_fun" pct (Eval (Vfptr b, pt) ty) te m E0)
+        | None => incontext (fun x => Evalof x ty) (step_expr LV pct l te m)
+        end
+    | RV, Eaddrof l ty =>
+        match is_loc l with
+        | Some (Lmem ofs t bf, ty') =>
+            match bf with Full => topred (Rred "red_addrof_loc" pct
+                                               (Eval (Vofptrsize (Ptrofs.unsigned ofs), t) ty) te m E0)
+                     | Bits _ _ _ _ => stuck
+            end
+        | Some (Ltmp _, _) => stuck
+        | Some (Lfun b pt, ty') =>
+            check type_eq ty ty';
+            topred (Rred "red_addrof_floc" pct (Eval (Vfptr b, pt) ty) te m E0)
+        | None =>
+            incontext (fun x => Eaddrof x ty) (step_expr LV pct l te m)
+        end
+    | RV, Eunop op r1 ty =>
+        match is_val r1 with
+        | Some(v1, vt1, ty1) =>
+            do v <- sem_unary_operation op v1 ty1 m;
+            at "failred_unop" trule pct',vt' <- UnopT op pct vt1;
+            topred (Rred "red_unop" pct' (Eval (v,vt') ty) te m E0)
+        | None =>
+            incontext (fun x => Eunop op x ty) (step_expr RV pct r1 te m)
+        end
+    | RV, Ebinop op r1 r2 ty =>
+        match is_val r1, is_val r2 with
+        | Some(v1, vt1, ty1), Some(v2, vt2, ty2) =>
+            do v <- sem_binary_operation (snd ge) op v1 ty1 v2 ty2 m;
+            at "failred_binop" trule pct',vt' <- BinopT op pct vt1 vt2;
+            topred (Rred "red_binop" pct' (Eval (v,vt') ty) te m E0) (* TODO: control points *)
+        | _, _ =>
+            incontext2 (fun x => Ebinop op x r2 ty) (step_expr RV pct r1 te m)
+                       (fun x => Ebinop op r1 x ty) (step_expr RV pct r2 te m)
+        end
+    | RV, Ecast r1 ty =>
+        match is_val r1 with
+        | Some(v1, vt1, ty1) =>
+            match ty1, ty with
+            | Tpointer _ _, Tpointer _ _ =>
+                do v <- sem_cast v1 ty1 ty m;
+                match v1, v with
+                | Vlong ofs1, Vlong ofs =>
+                    do w',tr1,_,lts1 <- do_deref_loc w ty1 m (Ptrofs.of_int64 ofs1) vt1 Full;
+                    do w'',tr,_,lts <- do_deref_loc w' ty m (Ptrofs.of_int64 ofs) vt1 Full;
+                    at "failred_cast_ptr_ptr" truletr (tr1++tr), pt' <- PPCastT pct vt1 lts1 lts ty;
+                    topred (Rred "red_cast_ptr_ptr" pct (Eval (v,pt') ty) te m (tr1++tr))
+                | _, _ => stuck
+                end
+            | Tpointer _ _, _ =>
+                do v <- sem_cast v1 ty1 ty m;
+                match v1 with
+                | Vlong ofs =>
+                    do w',tr,_,lts <- do_deref_loc w ty1 m (Ptrofs.of_int64 ofs) vt1 Full;
+                    at "failred_cast_ptr_int" truletr tr, pt' <- PICastT pct vt1 lts ty;
+                    topred (Rred "red_cast_ptr_int" pct (Eval (v,pt') ty) te m tr)
+                | _ => stuck
+                end
+            | _, Tpointer _ _ =>
+                do v <- sem_cast v1 ty1 ty m;
+                match v with
+                | Vlong ofs =>
+                    do w',tr,_,lts <- do_deref_loc w ty m (Ptrofs.of_int64 ofs) vt1 Full;
+                    at "failred_cast_int_ptr" truletr tr, pt' <- IPCastT pct vt1 lts ty;
+                    topred (Rred "red_cast_int_ptr" pct (Eval (v,pt') ty) te m tr)
+                | _ => stuck
+                end
+            | _, _ => 
+                do v <- sem_cast v1 ty1 ty m;
+                at "failred_cast_int_int" trule vt' <- IICastT pct vt1 ty;
+                topred (Rred "red_cast_int_int" pct (Eval (v,vt') ty) te m E0)
+            end
+        | None =>
+            incontext (fun x => Ecast x ty) (step_expr RV pct r1 te m)
+        end
+    | RV, Eseqand r1 r2 ty =>
+        match is_val r1 with
+        | Some(v1, vt1, ty1) =>
+            do b <- bool_val v1 ty1 m;
+            at "failred_seqand" trule pct' <- ExprSplitT pct vt1;
+            if b then topred (Rred "red_seqand_true" pct' (Eparen r2 type_bool ty) te m E0)
                else topred (Rred "red_seqand_false" pct' (Eval (Vint Int.zero,vt1) ty) te m E0)
-      | None =>
-          incontext (fun x => Eseqand x r2 ty) (step_expr RV pct r1 te m)
-      end
-  | RV, Eseqor r1 r2 ty =>
-      match is_val r1 with
-      | Some(v1, vt1, ty1) =>
-          do b <- bool_val v1 ty1 m;
-          trule pct' <- ExprSplitT pct vt1;
-          if b then topred (Rred "red_seqor_true" pct' (Eval (Vint Int.one, vt1) ty) te m E0)
-               else topred (Rred "red_seqor_false" pct' (Eparen r2 type_bool ty) te m E0)
-      | None =>
-          incontext (fun x => Eseqor x r2 ty) (step_expr RV pct r1 te m)
-      end
-  | RV, Econdition r1 r2 r3 ty =>
-      match is_val r1 with
-      | Some(v1, vt1, ty1) =>
-          do b <- bool_val v1 ty1 m;
-          trule pct' <- ExprSplitT pct vt1;
-          topred (Rred "red_condition" pct' (Eparen (if b then r2 else r3) ty ty) te m E0)
-      | None =>
-          incontext (fun x => Econdition x r2 r3 ty) (step_expr RV pct r1 te m)
-      end
-  | RV, Esizeof ty' ty =>
-      trule vt' <- ConstT pct;
-      topred (Rred "red_sizeof" pct (Eval (Vofptrsize (sizeof (snd ge) ty'), vt') ty) te m E0)
-  | RV, Ealignof ty' ty =>
-      trule vt' <- ConstT pct;
-      topred (Rred "red_alignof" pct (Eval (Vofptrsize (alignof (snd ge) ty'), vt') ty) te m E0)
-  | RV, Eassign l1 r2 ty =>
-      match is_loc l1, is_val r2 with
-      | Some (Lmem ofs pt1 bf, ty1), Some(v2, vt2, ty2) =>
-          check type_eq ty1 ty;
-          do v <- sem_cast v2 ty2 ty1 m;
-          do w',t,vvt,lts <- do_deref_loc w ty1 m ofs pt1 bf;
-          let (_,vt1) := vvt in
-          truletr t, pct',vt' <- AssignT pct vt1 vt2;
-          truletr t, pct'',vt'',lts' <- StoreT pct' pt1 vt' lts;
-          do w'',t',m',vvt' <- do_assign_loc w' ty1 m ofs pt1 bf (v,vt'') lts';
-          topred (Rred "red_assign_mem" pct'' (Eval vvt' ty) te m' (t ++ t'))
-      | Some (Ltmp b, ty1), Some (v2, vt2, ty2) =>
-          check type_eq ty1 ty;
-          do v1,vt1 <- te!b;
-          do v <- sem_cast v2 ty2 ty1 m;
-          trule pct',vt' <- AssignT pct vt1 vt2;
-          let te' := PTree.set b (v,vt') te in
-          topred (Rred "red_assign_tmp" pct' (Eval (v,vt') ty) te' m E0)
-      | Some (Lfun _ _, _), Some (v2, vt2, ty2) => stuck
-      | _, _ =>
-         incontext2 (fun x => Eassign x r2 ty) (step_expr LV pct l1 te m)
-                    (fun x => Eassign l1 x ty) (step_expr RV pct r2 te m)
-      end
-  | RV, Eassignop op l1 r2 tyres ty =>
-      match is_loc l1, is_val r2 with
-      | Some (Lmem ofs pt1 bf, ty1), Some(v2, vt2, ty2) =>
-          check type_eq ty1 ty;
-          do w',t,vvt,lts <- do_deref_loc w ty m ofs pt1 bf; (* anaaktge assn op *)
-          let (v1,vt1) := vvt in (* grabbing tag *)
-          truletr t, vt' <- LoadT pct pt1 vt1 lts; (* invoking the loadT rule *)
-          truletr t, vt'' <- AccessT pct vt';
-          let r' := Eassign (Eloc (Lmem ofs pt1 bf) ty1)
-                           (Ebinop op (Eval (v1,vt'') ty1) (Eval (v2,vt2) ty2) tyres) ty1 in
-          topred (Rred "red_assignop_mem" pct r' te m t)
-      | Some (Ltmp b, ty1), Some (v2, vt2, ty2) =>
-          check type_eq ty1 ty;
-          do v1,vt1 <- te!b;
-          trule vt' <- AccessT pct vt1;
-          let r' := Eassign (Eloc (Ltmp b) ty1)
-                           (Ebinop op (Eval (v1,vt') ty1) (Eval (v2,vt2) ty2) tyres) ty1 in
-          topred (Rred "red_assignop_tmp" pct r' te m E0)
-      | Some (Lfun b pt, ty1), Some(v2, vt2, ty2) =>
-          check type_eq ty1 ty;
-          let r' := Eassign (Eloc (Lfun b pt) ty1)
-                           (Ebinop op (Eval (Vfptr b,pt) ty1) (Eval (v2,vt2) ty2) tyres) ty1 in
-          topred (Rred "red_assignop_fun" pct r' te m E0)
-      | _, _ =>
-         incontext2 (fun x => Eassignop op x r2 tyres ty) (step_expr LV pct l1 te m)
-                    (fun x => Eassignop op l1 x tyres ty) (step_expr RV pct r2 te m)
-      end
-  | RV, Epostincr id l ty =>
-      match is_loc l with
-      | Some (Lmem ofs pt bf, ty1) =>
-          check type_eq ty1 ty;
-          do w',t, vvt, lts <- do_deref_loc w ty m ofs pt bf;
-          let (v,vt) := vvt in
-          truletr t, vt' <- LoadT pct pt vt lts;
-          truletr t, vt'' <- AccessT pct vt';
-          let op := match id with Incr => Oadd | Decr => Osub end in
-          let r' :=
-            Ecomma (Eassign (Eloc (Lmem ofs pt bf) ty)
-                            (Ebinop op (Eval (v,vt'') ty) (Econst (Vint Int.one) type_int32s) (incrdecr_type ty))
-                            ty)
-                   (Eval (v,vt'') ty) ty in
-          topred (Rred "red_postincr_mem" pct r' te m t)
-      | Some (Ltmp b, ty1) =>
-          check type_eq ty1 ty;
-          do v,vt <- te!b;
-          trule vt' <- AccessT pct vt;
-          let op := match id with Incr => Oadd | Decr => Osub end in
-          let r' := Ecomma (Eassign (Eloc (Ltmp b) ty)
-                            (Ebinop op (Eval (v,vt') ty)
-                                    (Econst (Vint Int.one) type_int32s) (incrdecr_type ty))
-                            ty)
-                    (Eval (v,vt') ty) ty in
-          topred (Rred "red_postincr_tmp" pct r' te m E0)
-      | Some (Lfun b pt, ty1) =>
-          check type_eq ty1 ty;
-          let op := match id with Incr => Oadd | Decr => Osub end in
-          let r' := Ecomma (Eassign (Eloc (Lfun b pt) ty1)
-                                    (Ebinop op (Eval (Vfptr b,pt) ty)
-                                            (Econst (Vint Int.one) type_int32s) (incrdecr_type ty))
-                                    ty)
-                    (Eval (Vfptr b,pt) ty) ty in
-          topred (Rred "red_postincr_fun" pct r' te m E0)
-      | not_loc =>
-          incontext (fun x => Epostincr id x ty) (step_expr LV pct l te m)
-      end
-  | RV, Ecomma r1 r2 ty =>
-      match is_val r1 with
-      | Some _ =>
-          check type_eq (typeof r2) ty;
-          topred (Rred "red_comma" pct r2 te m E0)
-      | None =>
-          incontext (fun x => Ecomma x r2 ty) (step_expr RV pct r1 te m)
-      end
-  | RV, Eparen r1 tycast ty =>
-      match is_val r1 with
-      | Some (v1, vt1, ty1) =>
-          do v <- sem_cast v1 ty1 tycast m;
-          trule pct',vt' <- ExprJoinT pct vt1;
-          topred (Rred "red_paren" pct' (Eval (v,vt') ty) te m E0)
-      | None =>
-          incontext (fun x => Eparen x tycast ty) (step_expr RV pct r1 te m)
-      end
-  | RV, Ecall r1 rargs ty =>
-      match is_val r1, is_val_list rargs with
-      | Some(vf, ft, tyf), Some vtl =>
-          match classify_fun tyf with
-          | fun_case_f tyargs tyres cconv =>
-              do fd <- Genv.find_funct (fst ge) vf;
-              do vargs <- sem_cast_arguments vtl tyargs m;
-              check type_eq (type_of_fundef fd) (Tfunction tyargs tyres cconv);
-              trule pct' <- CallT pct ft;
-              topred (Callred "red_call" fd vargs ty pct' te m)
-          | _ => stuck
-          end
-      | _, _ =>
-          incontext2 (fun x => Ecall x rargs ty) (step_expr RV pct r1 te m)
-                     (fun x => Ecall r1 x ty) (step_exprlist pct rargs te m)
-      end
-  | RV, Ebuiltin ef tyargs rargs ty =>
-      match is_val_list rargs with
-      | Some vtl =>
-          do vargs <- sem_cast_arguments vtl tyargs m;
-          match do_external ef w vargs pct m with
-          | None => stuck
-          | Some(w',t,v,pct', m') => topred (Rred "red_builtin" pct' (Eval v ty) te m' t)
-          end
-      | _ =>
-          incontext (fun x => Ebuiltin ef tyargs x ty) (step_exprlist pct rargs te m)
-      end
-  | _, _ => stuck
-  end
+        | None =>
+            incontext (fun x => Eseqand x r2 ty) (step_expr RV pct r1 te m)
+        end
+    | RV, Eseqor r1 r2 ty =>
+        match is_val r1 with
+        | Some(v1, vt1, ty1) =>
+            do b <- bool_val v1 ty1 m;
+            at "failred_seqor" trule pct' <- ExprSplitT pct vt1;
+            if b then topred (Rred "red_seqor_true" pct' (Eval (Vint Int.one, vt1) ty) te m E0)
+            else topred (Rred "red_seqor_false" pct' (Eparen r2 type_bool ty) te m E0)
+        | None =>
+            incontext (fun x => Eseqor x r2 ty) (step_expr RV pct r1 te m)
+        end
+    | RV, Econdition r1 r2 r3 ty =>
+        match is_val r1 with
+        | Some(v1, vt1, ty1) =>
+            do b <- bool_val v1 ty1 m;
+            at "failred_condition" trule pct' <- ExprSplitT pct vt1;
+            topred (Rred "red_condition" pct' (Eparen (if b then r2 else r3) ty ty) te m E0)
+        | None =>
+            incontext (fun x => Econdition x r2 r3 ty) (step_expr RV pct r1 te m)
+        end
+    | RV, Esizeof ty' ty =>
+        at "failred_sizeof" trule vt' <- ConstT pct;
+        topred (Rred "red_sizeof" pct (Eval (Vofptrsize (sizeof (snd ge) ty'), vt') ty) te m E0)
+    | RV, Ealignof ty' ty =>
+        at "failred_alignor" trule vt' <- ConstT pct;
+        topred (Rred "red_alignof" pct (Eval (Vofptrsize (alignof (snd ge) ty'), vt') ty) te m E0)
+    | RV, Eassign l1 r2 ty =>
+        match is_loc l1, is_val r2 with
+        | Some (Lmem ofs pt1 bf, ty1), Some(v2, vt2, ty2) =>
+            check type_eq ty1 ty;
+            do v <- sem_cast v2 ty2 ty1 m;
+            do w',t,vvt,lts <- do_deref_loc w ty1 m ofs pt1 bf;
+            let (_,vt1) := vvt in
+            at "failred_assign_mem1" truletr t, pct',vt' <- AssignT pct vt1 vt2;
+            at "failred_assign_mem2" truletr t, pct'',vt'',lts' <- StoreT pct' pt1 vt' lts;
+            do w'',t',m',vvt' <- do_assign_loc w' ty1 m ofs pt1 bf (v,vt'') lts';
+            topred (Rred "red_assign_mem" pct'' (Eval vvt' ty) te m' (t ++ t'))
+        | Some (Ltmp b, ty1), Some (v2, vt2, ty2) =>
+            check type_eq ty1 ty;
+            do v1,vt1 <- te!b;
+            do v <- sem_cast v2 ty2 ty1 m;
+            at "failred_assign_tmp" trule pct',vt' <- AssignT pct vt1 vt2;
+            let te' := PTree.set b (v,vt') te in
+            topred (Rred "red_assign_tmp" pct' (Eval (v,vt') ty) te' m E0)
+        | Some (Lfun _ _, _), Some (v2, vt2, ty2) => stuck
+        | _, _ =>
+            incontext2 (fun x => Eassign x r2 ty) (step_expr LV pct l1 te m)
+                       (fun x => Eassign l1 x ty) (step_expr RV pct r2 te m)
+        end
+    | RV, Eassignop op l1 r2 tyres ty =>
+        match is_loc l1, is_val r2 with
+        | Some (Lmem ofs pt1 bf, ty1), Some(v2, vt2, ty2) =>
+            check type_eq ty1 ty;
+            do w',t,vvt,lts <- do_deref_loc w ty m ofs pt1 bf; (* anaaktge assn op *)
+            let (v1,vt1) := vvt in (* grabbing tag *)
+            at "failred_assignop_mem1" truletr t, vt' <- LoadT pct pt1 vt1 lts; (* invoking the loadT rule *)
+            at "failred_assignop_mem2" truletr t, vt'' <- AccessT pct vt';
+            let r' := Eassign (Eloc (Lmem ofs pt1 bf) ty1)
+                              (Ebinop op (Eval (v1,vt'') ty1) (Eval (v2,vt2) ty2) tyres) ty1 in
+            topred (Rred "red_assignop_mem" pct r' te m t)
+        | Some (Ltmp b, ty1), Some (v2, vt2, ty2) =>
+            check type_eq ty1 ty;
+            do v1,vt1 <- te!b;
+            at "failred_assignop_tmp" trule vt' <- AccessT pct vt1;
+            let r' := Eassign (Eloc (Ltmp b) ty1)
+                              (Ebinop op (Eval (v1,vt') ty1) (Eval (v2,vt2) ty2) tyres) ty1 in
+            topred (Rred "red_assignop_tmp" pct r' te m E0)
+        | Some (Lfun b pt, ty1), Some(v2, vt2, ty2) =>
+            check type_eq ty1 ty;
+            let r' := Eassign (Eloc (Lfun b pt) ty1)
+                              (Ebinop op (Eval (Vfptr b,pt) ty1) (Eval (v2,vt2) ty2) tyres) ty1 in
+            topred (Rred "red_assignop_fun" pct r' te m E0)
+        | _, _ =>
+            incontext2 (fun x => Eassignop op x r2 tyres ty) (step_expr LV pct l1 te m)
+                       (fun x => Eassignop op l1 x tyres ty) (step_expr RV pct r2 te m)
+        end
+    | RV, Epostincr id l ty =>
+        match is_loc l with
+        | Some (Lmem ofs pt bf, ty1) =>
+            check type_eq ty1 ty;
+            do w',t, vvt, lts <- do_deref_loc w ty m ofs pt bf;
+            let (v,vt) := vvt in
+            at "failred_postincr_mem1" truletr t, vt' <- LoadT pct pt vt lts;
+            at "failred_postincr_mem2" truletr t, vt'' <- AccessT pct vt';
+            let op := match id with Incr => Oadd | Decr => Osub end in
+            let r' :=
+              Ecomma (Eassign (Eloc (Lmem ofs pt bf) ty)
+                              (Ebinop op (Eval (v,vt'') ty) (Econst (Vint Int.one) type_int32s)
+                                      (incrdecr_type ty)) ty)
+                     (Eval (v,vt'') ty) ty in
+            topred (Rred "red_postincr_mem" pct r' te m t)
+        | Some (Ltmp b, ty1) =>
+            check type_eq ty1 ty;
+            do v,vt <- te!b;
+            at "failred_postincr_tmp" trule vt' <- AccessT pct vt;
+            let op := match id with Incr => Oadd | Decr => Osub end in
+            let r' := Ecomma (Eassign (Eloc (Ltmp b) ty)
+                                      (Ebinop op (Eval (v,vt') ty)
+                                              (Econst (Vint Int.one) type_int32s)
+                                              (incrdecr_type ty)) ty)
+                             (Eval (v,vt') ty) ty in
+            topred (Rred "red_postincr_tmp" pct r' te m E0)
+        | Some (Lfun b pt, ty1) =>
+            check type_eq ty1 ty;
+            let op := match id with Incr => Oadd | Decr => Osub end in
+            let r' := Ecomma (Eassign (Eloc (Lfun b pt) ty1)
+                                      (Ebinop op (Eval (Vfptr b,pt) ty)
+                                              (Econst (Vint Int.one) type_int32s)
+                                              (incrdecr_type ty)) ty)
+                             (Eval (Vfptr b,pt) ty) ty in
+            topred (Rred "red_postincr_fun" pct r' te m E0)
+        | not_loc =>
+            incontext (fun x => Epostincr id x ty) (step_expr LV pct l te m)
+        end
+    | RV, Ecomma r1 r2 ty =>
+        match is_val r1 with
+        | Some _ =>
+            check type_eq (typeof r2) ty;
+            topred (Rred "red_comma" pct r2 te m E0)
+        | None =>
+            incontext (fun x => Ecomma x r2 ty) (step_expr RV pct r1 te m)
+        end
+    | RV, Eparen r1 tycast ty =>
+        match is_val r1 with
+        | Some (v1, vt1, ty1) =>
+            do v <- sem_cast v1 ty1 tycast m;
+            at "failred_paren" trule pct',vt' <- ExprJoinT pct vt1;
+            topred (Rred "red_paren" pct' (Eval (v,vt') ty) te m E0)
+        | None =>
+            incontext (fun x => Eparen x tycast ty) (step_expr RV pct r1 te m)
+        end
+    | RV, Ecall r1 rargs ty =>
+        match is_val r1, is_val_list rargs with
+        | Some(vf, ft, tyf), Some vtl =>
+            match classify_fun tyf with
+            | fun_case_f tyargs tyres cconv =>
+                do fd <- Genv.find_funct (fst ge) vf;
+                do vargs <- sem_cast_arguments vtl tyargs m;
+                check type_eq (type_of_fundef fd) (Tfunction tyargs tyres cconv);
+                at "failred_call" trule pct' <- CallT pct ft;
+                topred (Callred "red_call" fd vargs ty pct' te m)
+            | _ => stuck
+            end
+        | _, _ =>
+            incontext2 (fun x => Ecall x rargs ty) (step_expr RV pct r1 te m)
+                       (fun x => Ecall r1 x ty) (step_exprlist pct rargs te m)
+        end
+    | RV, Ebuiltin ef tyargs rargs ty =>
+        match is_val_list rargs with
+        | Some vtl =>
+            do vargs <- sem_cast_arguments vtl tyargs m;
+            match do_external ef w vargs pct m with
+            | None => stuck
+            | Some(w',t,v,pct', m') => topred (Rred "red_builtin" pct' (Eval v ty) te m' t)
+            end
+        | _ =>
+            incontext (fun x => Ebuiltin ef tyargs x ty) (step_exprlist pct rargs te m)
+        end
+    | _, _ => stuck
+    end
 
-with step_exprlist (pct: tag) (rl: exprlist) (te: tenv) (m: mem): reducts exprlist :=
-  match rl with
-  | Enil =>
-      nil
-  | Econs r1 rs =>
-      incontext2 (fun x => Econs x rs) (step_expr RV pct r1 te m)
-                 (fun x => Econs r1 x) (step_exprlist pct rs te m)
-  end.
+  with step_exprlist (pct: tag) (rl: exprlist) (te: tenv) (m: mem): reducts exprlist :=
+         match rl with
+         | Enil =>
+             nil
+         | Econs r1 rs =>
+             incontext2 (fun x => Econs x rs) (step_expr RV pct r1 te m)
+                        (fun x => Econs r1 x) (step_exprlist pct rs te m)
+         end.
 
-(** Technical properties on safe expressions. *)
-Inductive imm_safe_t: kind -> expr -> tag -> tenv -> mem -> Prop :=
+  (** Technical properties on safe expressions. *)
+  Inductive imm_safe_t: kind -> expr -> tag -> tenv -> mem -> Prop :=
   | imm_safe_t_val: forall v ty pct te m,
       imm_safe_t RV (Eval v ty) pct te m
   | imm_safe_t_loc: forall l ty pct te m,
@@ -1271,8 +1087,16 @@ Inductive imm_safe_t: kind -> expr -> tag -> tenv -> mem -> Prop :=
       lred ge e l pct te m l' te' m' ->
       context LV to C ->
       imm_safe_t to (C l) pct te m
+  | imm_safe_t_lfailred: forall to C l pct te m msg params,
+      lfailred ge l pct msg params ->
+      context LV to C ->
+      imm_safe_t to (C l) pct te m
   | imm_safe_t_rred: forall to C pct r te m t pct' r' te' m' w',
       rred ge pct r te m t pct' r' te' m' -> possible_trace w t w' ->
+      context RV to C ->
+      imm_safe_t to (C r) pct te m
+  | imm_safe_t_rfailred: forall to C r pct te m tr msg params w',
+      rfailred ge pct r te m tr msg params -> possible_trace w tr w' ->
       context RV to C ->
       imm_safe_t to (C r) pct te m
   | imm_safe_t_callred: forall to C pct pct' r te m fd args ty,
@@ -1287,7 +1111,9 @@ Proof.
   constructor.
   constructor.
   eapply imm_safe_lred; eauto.
+  eapply imm_safe_lfailred; eauto.
   eapply imm_safe_rred; eauto.
+  eapply imm_safe_rfailred; eauto.
   eapply imm_safe_callred; eauto.
 Qed.
 
@@ -1300,7 +1126,6 @@ Fixpoint exprlist_all_values (rl: exprlist) : Prop :=
 
 Definition invert_expr_prop (a: expr) (pct: tag) (te: tenv) (m: mem) : Prop :=
   match a with
-  | Econst v ty => exists vt', ConstT pct = PolicySuccess vt'
   | Eloc l ty => False
   | Evar x ty =>
       e!x = Some PRIV
@@ -1341,6 +1166,26 @@ Definition invert_expr_prop (a: expr) (pct: tag) (te: tenv) (m: mem) : Prop :=
       exists v, sem_unary_operation op v1 ty1 m = Some v
   | Ebinop op (Eval (v1,vt1) ty1) (Eval (v2,vt2) ty2) ty =>
       exists v, sem_binary_operation (snd ge) op v1 ty1 v2 ty2 m = Some v
+  | Ecast (Eval (v1,vt1) (Tpointer ty1 attr1)) (Tpointer ty attr) =>
+      exists v ofs1 ofs tr1 w' v2 vt2 lts1 tr w'' v3 vt3 lts,
+      sem_cast v1 (Tpointer ty1 attr1) (Tpointer ty attr) m = Some v /\
+        v1 = Vlong ofs1 /\ v = Vlong ofs /\
+        deref_loc ge (Tpointer ty1 attr1) m (Ptrofs.of_int64 ofs1) vt1 Full tr1 (v2,vt2) lts1 /\
+        possible_trace w tr1 w' /\
+        deref_loc ge (Tpointer ty attr) m (Ptrofs.of_int64 ofs) vt1 Full tr (v3,vt3) lts /\
+        possible_trace w' tr w''
+  | Ecast (Eval (v1,vt1) (Tpointer ty1 attr1)) ty =>
+      exists v ofs1 tr1 w' v2 vt2 lts1,
+      sem_cast v1 (Tpointer ty1 attr1) ty m = Some v /\
+        v1 = Vlong ofs1 /\
+        deref_loc ge (Tpointer ty1 attr1) m (Ptrofs.of_int64 ofs1) vt1 Full tr1 (v2,vt2) lts1 /\
+        possible_trace w tr1 w'
+  | Ecast (Eval (v1,vt1) ty1) (Tpointer ty attr) =>
+      exists v ofs tr w' v2 vt2 lts,
+      sem_cast v1 ty1 (Tpointer ty attr) m = Some v /\
+        v = Vlong ofs /\
+        deref_loc ge (Tpointer ty attr) m (Ptrofs.of_int64 ofs) vt1 Full tr (v2,vt2) lts /\
+        possible_trace w tr w'
   | Ecast (Eval (v1,vt1) ty1) ty =>
       exists v, sem_cast v1 ty1 ty m = Some v
   | Eseqand (Eval (v1,vt1) ty1) r2 ty =>
@@ -1350,17 +1195,17 @@ Definition invert_expr_prop (a: expr) (pct: tag) (te: tenv) (m: mem) : Prop :=
   | Econdition (Eval (v1,vt1) ty1) r1 r2 ty =>
       exists b, bool_val v1 ty1 m = Some b
   | Eassign (Eloc (Lmem ofs pt bf) ty1) (Eval (v2,vt2) ty2) ty =>
-      exists v1 v2' v2'' m' vt1 vt2' vt' vt'' pct' pct'' t t' w' w'' lts lts',
+      exists v1 v2' vt1 t w' lts,
       ty = ty1 /\ sem_cast v2 ty2 ty1 m = Some v2' /\
         deref_loc ge ty1 m ofs pt bf t (v1,vt1) lts /\ possible_trace w t w' /\
-        AssignT pct vt1 vt2 = PolicySuccess (pct', vt2') /\
-        StoreT pct' pt vt2' lts = PolicySuccess (pct'', vt', lts') /\
-        assign_loc ge ty1 m ofs pt bf (v2',vt') t' m' (v2'',vt'') lts' /\ possible_trace w' t' w''
+        (forall pct' vt2' pct'' vt' lts',
+            AssignT pct vt1 vt2 = PolicySuccess (pct', vt2') ->
+            StoreT pct' pt vt2' lts = PolicySuccess (pct'', vt', lts') ->
+            exists m' t' v2'' vt'' w'', assign_loc ge ty1 m ofs pt bf (v2',vt') t' m' (v2'',vt'') lts' /\ possible_trace w' t' w'')
   | Eassign (Eloc (Ltmp b) ty1) (Eval (v2,vt2) ty2) ty =>
-      exists v1 v2' vt1 vt' pct',
-      ty = ty1 /\ te!b = Some (v1,vt1) /\ sem_cast v2 ty2 ty1 m = Some v2' /\
-        AssignT pct vt1 vt2 = PolicySuccess (pct', vt')
-  | Eassign (Eloc (Lfun _ _) _) _ ty => False
+      exists v1 v2' vt1,
+      ty = ty1 /\ te!b = Some (v1,vt1) /\ sem_cast v2 ty2 ty1 m = Some v2'
+  | Eassign (Eloc (Lfun _ _) _) (Eval _ _) ty => False
   | Ecomma (Eval v ty1) r2 ty =>
       typeof r2 = ty
   | Eparen (Eval (v1,vt1) ty1) tycast ty =>
@@ -1374,7 +1219,7 @@ Definition invert_expr_prop (a: expr) (pct: tag) (te: tenv) (m: mem) : Prop :=
       /\ type_of_fundef fd = Tfunction tyargs tyres cconv
   | Ebuiltin ef tyargs rargs ty =>
       exprlist_all_values rargs ->
-      exists vargs t vres pct pct' m' w',
+      exists vargs t vres pct' m' w',
          cast_arguments m rargs tyargs vargs
       /\ external_call ef (fst ge) vargs pct m t vres pct' m'
       /\ possible_trace w t w'
@@ -1394,32 +1239,53 @@ Proof.
   - exists co, delta, bf; auto.
 Qed.
 
+Lemma lfailred_invert:
+  forall l pct te m msg param, lfailred ge l pct msg param -> invert_expr_prop l pct te m.
+Proof.
+  induction 1; red; auto.
+  - exists co, delta, bf; auto.
+  - exists co, delta, bf; auto.
+Qed.
+
+Ltac chomp :=
+  match goal with
+  | [H: possible_trace _ (?t1 ++ ?t2) _ |- _] =>
+      let w' := fresh "w" in
+      let H1 := fresh "H" in
+      let H2 := fresh "H" in
+      apply possible_trace_app_inv in H;
+      destruct H as [w' [H1 H2]]
+  | [H1: ?rule = PolicySuccess _, H2: ?rule = PolicyFail _ _ |- _] =>
+      rewrite H1 in H2; discriminate
+  | [H1: ?rule = PolicySuccess _, H2: ?rule = PolicySuccess _ |- _] =>
+      rewrite H1 in H2; inv H2
+  | [H1: forall _ _, ?ty <> Tpointer _ _, H2: ?ty = Tpointer _ _ |- _] =>
+      congruence
+  | _ => idtac
+  end.
+
 Lemma rred_invert:
   forall w' pct r te m t pct' r' te' m', rred ge pct r te m t pct' r' te' m' -> possible_trace w t w' -> invert_expr_prop r pct te m.
 Proof.
-  induction 1; intros; red; auto.
-  - exists vt'; auto.
-  - exists tr, v, vt, w', lts; auto.
-  - exists v, vt; auto.
-  - exists v; auto.
-  - exists v; auto.
-  - exists v; auto.
-  - exists true; auto.
-  - exists false; auto.
-  - exists true; auto.
-  - exists false; auto.
-  - exists b; auto.
-  - exists v1, v', v'', m', vt1, vt', vt'', vt''', PCT', PCT'', t1, t2.
-    apply possible_trace_app_inv in H4. destruct H4 as [w0 H4].
-    destruct H4.
-    exists w0, w', lts, lts'; repeat split; auto.
-  - exists v1, v, vt1, vt', PCT'; repeat split; auto.
-  - exists t0, v1, vt1, w', lts; auto.
-  - exists v1, vt1; auto.
-  - exists t0, v, vt, w', lts; auto.
-  - exists v, vt; auto.
-  - exists v; auto.
-  - intros. exists vargs, t0, vres, pct, PCT', m', w'; auto.
+  induction 1; intros; red; auto; repeat (repeat chomp; eexists; eauto; intros).
+  - destruct ty1; destruct ty; try congruence; repeat (eexists; eauto). 
+  - destruct ty1; destruct ty; try congruence; repeat (eexists; eauto). 
+  - destruct ty1; destruct ty; try congruence; repeat (eexists; eauto). 
+  - destruct ty1; destruct ty; try congruence.
+    eapply possible_trace_app_inv in H7 as [w0 [P Q]].
+    repeat (eexists; eauto). 
+Qed.
+
+Lemma rfailred_invert:
+  forall w' pct r te m tr msg params, rfailred ge pct r te m tr msg params -> possible_trace w tr w' -> invert_expr_prop r pct te m.
+Proof.
+  induction 1; intros; red; auto; repeat (repeat chomp; eexists; eauto; intros).
+  - destruct ty1; destruct ty; try congruence; repeat (eexists; eauto).
+  - destruct ty1; destruct ty; try congruence; repeat (eexists; eauto).
+  - destruct ty1; destruct ty; try congruence; repeat (eexists; eauto).
+  - destruct ty1; destruct ty; try congruence.
+    eapply possible_trace_app_inv in H7 as [w0 [P Q]].
+    repeat (eexists; eauto). 
 Qed.
 
 Lemma callred_invert:
@@ -1448,13 +1314,13 @@ Proof.
   apply context_contextlist_ind; intros; try (exploit H0; [eauto|intros]); simpl; auto;
     try (destruct (C a); auto; contradiction).
   - destruct e1; auto; destruct (C a); destruct v; auto. destruct v0; auto; contradiction.
-  - destruct e1; auto. destruct l; auto.
-    destruct (C a); auto; destruct v; auto. admit. admit. admit.
+  - destruct e1; auto.
+    destruct l; auto; destruct (C a); auto; destruct v; auto; inv H2.
   - destruct e1; auto; destruct (C a); auto; destruct l; auto; contradiction.
   - destruct e1; auto. destruct v. intros. elim (H0 a pct te m); auto.
   - intros. elim (H0 a pct te m); auto.
   - red; intros. destruct e1; auto. elim (H0 a pct te m); auto.
-Admitted.
+Qed.
 
 Lemma imm_safe_t_inv:
   forall k a pct te m,
@@ -1470,8 +1336,14 @@ Proof.
   - assert (invert_expr_prop (C l) pct te m).
     { eapply A; eauto. eapply lred_invert; eauto. }
     red in H. destruct (C l); auto; contradiction.
+  - assert (invert_expr_prop (C l) pct te m).
+    { eapply A; eauto. eapply lfailred_invert; eauto. }
+    red in H. destruct (C l); auto; contradiction.
   - assert (invert_expr_prop (C r) pct te m).
     { eapply A; eauto. eapply rred_invert; eauto. }
+    red in H. destruct (C r); auto; contradiction.
+  - assert (invert_expr_prop (C r) pct te m).
+    { eapply A; eauto. eapply rfailred_invert; eauto. }
     red in H. destruct (C r); auto; contradiction.
   - assert (invert_expr_prop (C r) pct te m).
     { eapply A; eauto. eapply callred_invert; eauto. }
@@ -1505,8 +1377,8 @@ Definition reduction_ok (k: kind) (pct: tag) (a: expr) (te: tenv) (m: mem) (rd: 
   | RV, Callred _ fd args tyres pct' te' m' => callred ge pct a m pct' fd args tyres /\ te' = te /\ m' = m
   | LV, Stuckred => ~imm_safe_t k a pct te m
   | RV, Stuckred => ~imm_safe_t k a pct te m
-  | LV, Failstopred msg params tr => lfailred ge a pct msg params /\ tr = E0
-  | RV, Failstopred msg params tr => rfailred ge pct a te m tr msg params
+  | LV, Failstopred _ msg params tr => lfailred ge a pct msg params /\ tr = E0
+  | RV, Failstopred _ msg params tr => rfailred ge pct a te m tr msg params
   | _, _ => False
   end.
 
@@ -1540,25 +1412,23 @@ Lemma sem_cast_arguments_sound:
   is_val_list rargs = Some vtl ->
   sem_cast_arguments vtl tyargs m = Some vargs ->
   cast_arguments m rargs tyargs vargs.
-Admitted.
-(*Proof.
+Proof.
   induction rargs; simpl; intros.
   inv H. destruct tyargs; simpl in H0; inv H0. constructor.
-  monadInv. inv H. simpl in H0. destruct p as [v1 t1]. destruct tyargs; try congruence. monadInv.
+  monadInv. inv H. simpl in H0. destruct p as [[v1 t1] ty1]. destruct tyargs; try congruence. monadInv.
   inv H0. rewrite (is_val_inv _ _ _ Heqo). constructor. auto. eauto.
-Qed.*)
+Qed.
 
 Lemma sem_cast_arguments_complete:
   forall m al tyl vl,
   cast_arguments m al tyl vl ->
   exists vtl, is_val_list al = Some vtl /\ sem_cast_arguments vtl tyl m = Some vl.
-Admitted.
-(*Proof.
+Proof.
   induction 1.
-  exists (@nil (val * type)); auto.
+  exists (@nil (atom * type)); auto.
   destruct IHcast_arguments as [vtl [A B]].
-  exists ((v, ty) :: vtl); simpl. rewrite A; rewrite B; rewrite H. auto.
-Qed.*)
+  exists (((v,vt), ty) :: vtl); simpl. rewrite A; rewrite B; rewrite H. auto.
+Qed.
 
 Lemma topred_ok:
   forall k pct a m te rd,
@@ -1697,13 +1567,12 @@ Qed.
 
 Lemma is_val_list_all_values:
   forall al vtl, is_val_list al = Some vtl -> exprlist_all_values al.
-Admitted.
-(*Proof.
-  induction al; simpl; intros. auto.
-  destruct (is_val r1) as [[v ty]|] eqn:?; try discriminate.
-  destruct (is_val_list al) as [vtl'|] eqn:?; try discriminate.
+Proof.
+  induction al0; simpl; intros; auto.
+  destruct (is_val r1) as [[[v vt] ty]|] eqn:?; try discriminate.
+  destruct (is_val_list al0) as [vtl'|] eqn:?; try discriminate.
   rewrite (is_val_inv _ _ _ Heqo). eauto.
-Qed.*)
+Qed.
 
 Ltac myinv :=
   match goal with
@@ -1716,67 +1585,142 @@ Ltac myinv :=
 
 Ltac tagdestr :=
   match goal with
-  | [ |- context [trule _ <- FieldT ?ge ?pct ?pt ?ty ?id; _]] =>
+  | [ |- context [at ?rule trule _ <- FieldT ?ge ?pct ?pt ?ty ?id; _]] =>
       let E := fresh "E" in
       let pt' := fresh "pt" in
       destruct (FieldT ge pct pt ty id) as [pt'|msg params] eqn:E
-  | [ |- context [trule _ <- ConstT ?pct; _]] =>
+  | [ |- context [at ?rule trule _ <- ConstT ?pct; _]] =>
       let E := fresh "E" in
       let vt' := fresh "vt" in
       destruct (ConstT pct) as [vt'|msg params] eqn:E
-  | [ |- context [truletr _, _ <- LoadT ?pct ?pt ?vt ?lts; _]] =>
+  | [ |- context [at ?rule truletr _, _ <- LoadT ?pct ?pt ?vt ?lts; _]] =>
       let E := fresh "E" in
       let vt' := fresh "vt" in
       destruct (LoadT pct pt vt lts) as [vt'|msg params] eqn:E     
-  | [ |- context [truletr _, _ <- AccessT ?pct ?vt; _]] =>
+  | [ |- context [at ?rule truletr _, _ <- AccessT ?pct ?vt; _]] =>
       let E := fresh "E" in
       let vt' := fresh "vt" in
       destruct (AccessT pct vt) as [vt'|msg params] eqn:E
-  | [ |- context [trule _ <- UnopT ?op ?pct ?vt; _]] =>
+  | [ |- context [at ?rule trule _ <- UnopT ?op ?pct ?vt; _]] =>
       let E := fresh "E" in
       let pct' := fresh "pct" in
       let vt' := fresh "vt" in
       destruct (UnopT op pct vt) as [[pct' vt']|msg params] eqn:E
-  | [ |- context [trule _ <- BinopT ?op ?pct ?vt1 ?vt2; _]] =>
+  | [ |- context [at ?rule trule _ <- BinopT ?op ?pct ?vt1 ?vt2; _]] =>
       let E := fresh "E" in
       let pct' := fresh "pct" in
       let vt' := fresh "vt" in
       destruct (BinopT op pct vt1 vt2) as [[pct' vt']|msg params] eqn:E
-  | [ |- context [trule _ <- ExprSplitT ?pct ?vt; _]] =>
+  | [ |- context [at ?rule trule _ <- ExprSplitT ?pct ?vt; _]] =>
       let E := fresh "E" in
       let pct' := fresh "pct" in
       destruct (ExprSplitT pct) as [pct'|msg params] eqn:E
-  | [ |- context [truletr _, _ <- AssignT ?pct ?vt ?vt'; _]] =>
+  | [ |- context [at ?rule truletr _, _ <- AssignT ?pct ?vt ?vt'; _]] =>
       let E := fresh "E" in
       let pct' := fresh "pct" in
       let vt'' := fresh "vt" in
       destruct (AssignT pct vt vt') as [[pct' vt'']|msg params] eqn:E  
-  | [ |- context [truletr _, _ <- StoreT ?pct ?pt ?vt ?lts; _]] =>
+  | [ |- context [at ?rule truletr _, _ <- StoreT ?pct ?pt ?vt ?lts; _]] =>
       let E := fresh "E" in
       let pct' := fresh "pct" in
       let vt' := fresh "vt" in
       let lts' := fresh "lts" in
       destruct (StoreT pct pt vt lts) as [[[pct' vt'] lts']|msg params] eqn:E
-  | [ |- context [trule _ <- CallT ?pct ?pt; _]] =>
+  | [ |- context [at ?rule trule _ <- CallT ?pct ?pt; _]] =>
       let E := fresh "E" in
       let pct' := fresh "pct" in
       destruct (CallT pct pt) as [pct'|msg params] eqn:E
-  | [ |- context [trule _ <- ExprJoinT ?pct ?vt; _]] =>
+  | [ |- context [at ?rule trule _ <- ExprJoinT ?pct ?vt; _]] =>
       let E := fresh "E" in
       let pct' := fresh "pct" in
       let vt' := fresh "vt" in
       destruct (ExprJoinT pct vt) as [[pct' vt']|msg params] eqn:E
+  | [ |- context [at ?rule trule _ <- IICastT ?pct ?vt ?ty; _]] =>
+      let vt' := fresh "vt" in
+      destruct (IICastT pct vt ty) as [vt'|msg params] eqn:?
+  | [ |- context [at ?rule truletr _, _ <- PICastT ?pct ?pt ?lts ?ty; _]] =>
+      let vt' := fresh "vt" in
+      destruct (PICastT pct pt lts ty) as [vt'|msg params] eqn:?
+  | [ |- context [at ?rule truletr _, _ <- IPCastT ?pct ?vt ?lts (Tpointer ?ty ?a); _]] =>
+      let pt' := fresh "pt" in
+      destruct (IPCastT pct vt lts (Tpointer ty a)) as [pt'|msg params] eqn:?
+  | [ |- context [at ?rule truletr _, _ <- PPCastT ?pct ?pt ?lts1 ?lts2 ?ty; _]] =>
+      let pt' := fresh "pt" in
+      destruct (PPCastT pct pt lts1 lts2 ty) as [pt'|msg params] eqn:?
   | _ => idtac
   end.
 
 Ltac tagdestr_ok := tagdestr; [| apply topred_ok; try split; econstructor; eauto].
 
+Definition is_pointer (ty : type) : option (type * attr) :=
+  match ty with
+  | Tpointer ty' attr => Some (ty', attr)
+  | _ => None
+  end.
+
+Lemma is_pointer_inv :
+  forall ty ty' attr,
+    is_pointer ty = Some (ty', attr) ->
+    ty = Tpointer ty' attr.
+Proof.
+  destruct ty; simpl; congruence.
+Qed.
+
+Ltac do_do :=
+  match goal with
+  | [ H1: deref_loc _ _ _ _ _ _ ?tr _ _, H2: possible_trace _ ?tr _ |- _] =>
+      eapply do_deref_loc_complete in H1; eauto
+  | _ => idtac
+  end.
+
+Ltac dodestr :=
+  match goal with
+  | [ |- context [match ?e with
+                  | Some _ => _
+                  | _ => _
+                  end] ] =>
+      destruct e eqn:?
+  | [ |- exists w', possible_trace ?w E0 w' ] =>
+      exists w; constructor
+  | [ |- context [match ?v with
+                  | Vlong _ => _
+                  | _ => _
+                  end] ] => destruct v
+  | [ |- context [let '(_, _) := ?e in _] ] =>
+      destruct e
+  | [ H: do_deref_loc _ _ _ _ _ _ = Some (_, _, ?a, _) |- _ ] =>
+      destruct a; eapply do_deref_loc_sound in H as [? ?]
+  | _ => idtac
+  end.
+
+Ltac solve_red :=
+  match goal with
+  | [ |- reducts_ok _ _ _ _ _ (topred (Rred "red_cast_int_int" _ _ _ _ _)) ] =>
+      eapply topred_ok; auto; split; [eapply red_cast_int_int|]
+  | [ |- reducts_ok _ _ _ _ _ (failred "failred_cast_int_int" _ _ _) ] =>
+      eapply topred_ok; auto; eapply failred_cast_int_int
+  | [ |- reducts_ok _ _ _ _ _ (topred (Rred "red_cast_ptr_int" _ _ _ _ _)) ] =>
+      eapply topred_ok; auto; split; [eapply red_cast_ptr_int|]
+  | [ |- reducts_ok _ _ _ _ _ (failred "failred_cast_ptr_int" _ _ _) ] =>
+      eapply topred_ok; auto; eapply failred_cast_ptr_int
+  | [ |- reducts_ok _ _ _ _ _ (topred (Rred "red_cast_int_ptr" _ _ _ _ _)) ] =>
+      eapply topred_ok; auto; split; [eapply red_cast_int_ptr|]
+  | [ |- reducts_ok _ _ _ _ _ (failred "failred_cast_int_ptr" _ _ _) ] =>
+      eapply topred_ok; auto; eapply failred_cast_int_ptr
+  | [ |- reducts_ok _ _ _ _ _ (topred (Rred "red_cast_ptr_ptr" _ _ _ _ _)) ] =>
+      eapply topred_ok; auto; split; [eapply red_cast_ptr_ptr|]
+  | [ |- reducts_ok _ _ _ _ _ (failred "failred_cast_ptr_ptr" _ _ _) ] =>
+      eapply topred_ok; auto; eapply failred_cast_ptr_ptr
+  end.
+
 Theorem step_expr_sound:
   forall pct a k te m, reducts_ok k pct a te m (step_expr k pct a te m)
 with step_exprlist_sound:
   forall pct al te m, list_reducts_ok pct al te m (step_exprlist pct al te m).
-Proof with (try (apply not_invert_ok; simpl; intro; myinv; intuition congruence; fail)).
-  - induction a; intros; simpl; destruct k; try (apply wrong_kind_ok; simpl; congruence).
+Proof with (try (apply not_invert_ok; simpl; intro; myinv; repeat do_do; intuition congruence; fail)).
+  Opaque do_deref_loc. Opaque do_assign_loc.
+  - clear step_expr_sound.
+    induction a; intros; simpl; destruct k; try (apply wrong_kind_ok; simpl; congruence).
     + (* Eval *)
       split; intros. tauto. simpl; congruence.
     + (* Evar *)
@@ -1809,13 +1753,11 @@ Proof with (try (apply not_invert_ok; simpl; intro; myinv; intuition congruence;
       * (* Lmem *)
         rewrite (is_loc_inv _ _ _ Heqo).
         destruct (type_eq ty ty')... subst ty'.
-        destruct (do_deref_loc w ty m ofs pt bf) as [[[[w' t] [v vt]] lts] | ] eqn:?.
-        -- exploit do_deref_loc_sound; eauto. intros [A B].
-           tagdestr; [| apply topred_ok; eapply failred_rvalof_mem1; eauto].
-           tagdestr; [| apply topred_ok; eapply failred_rvalof_mem2; eauto].
-           apply topred_ok; auto. red. split. eapply red_rvalof_mem; eauto. exists w'; auto.
-        -- apply not_invert_ok. simpl; intros; myinv. exploit do_deref_loc_complete; eauto.
-           congruence.
+        destruct (do_deref_loc w ty m ofs pt bf) as [[[[w' t] [v vt]] lts] | ] eqn:?...
+        exploit do_deref_loc_sound; eauto. intros [A B].
+        tagdestr; [| apply topred_ok; eapply failred_rvalof_mem1; eauto].
+        tagdestr; [| apply topred_ok; eapply failred_rvalof_mem2; eauto].
+        apply topred_ok; auto. red. split. eapply red_rvalof_mem; eauto. exists w'; auto.
       * (* Ltmp *)
         rewrite (is_loc_inv _ _ _ Heqo).
         destruct (type_eq ty ty')... subst ty'.
@@ -1870,10 +1812,12 @@ Proof with (try (apply not_invert_ok; simpl; intro; myinv; intuition congruence;
         eapply incontext2_ok; eauto.
       * eapply incontext2_ok; eauto.
     + (* cast *)
-      destruct (is_val a) as [[[v vt] ty'] | ] eqn:?. rewrite (is_val_inv _ _ _ Heqo).
-      * (* top *)
-        destruct (sem_cast v ty' ty m) as [v'|] eqn:?...
-        apply topred_ok; auto. split. apply red_cast; auto. exists w; constructor.
+      destruct (is_val a) as [[[v vt] ty1] | ] eqn:?.
+      * rewrite (is_val_inv _ _ _ Heqo).
+        destruct ty1 eqn:?; destruct ty eqn:?;
+                 repeat (repeat (dodestr; tagdestr);
+                         try solve_red; try congruence; eauto)...
+        exists w1. eapply possible_trace_app; eauto.
       * (* depth *)
         eapply incontext_ok; eauto.
     + (* seqand *)
@@ -1911,24 +1855,23 @@ Proof with (try (apply not_invert_ok; simpl; intro; myinv; intuition congruence;
         destruct (type_eq ty1 ty)... subst ty1.
         destruct (sem_cast v2 ty2 ty m) as [v|] eqn:?...
         destruct (do_deref_loc w ty m ofs pt bf) as [[[[w' t] [v' vt]] lts] | ] eqn:?...
-        -- exploit do_deref_loc_sound; eauto. intros [R S].
-           tagdestr; [| apply topred_ok; eapply failred_assign_mem1; eauto].
-           tagdestr; [| apply topred_ok; eapply failred_assign_mem2; eauto].
-           destruct (do_assign_loc w' ty m ofs pt bf (v,vt1) lts0) as [[[[w'' t'] m'] [v'' vt']]|] eqn:?.
-           ++ exploit do_assign_loc_sound; eauto. intros [P Q].
-              apply topred_ok; auto.
-              split. inversion P; subst; eapply red_assign_mem; eauto.
-              exists w''. eapply possible_trace_app; eauto.
-           ++ apply not_invert_ok; simpl; intros. myinv.
-              exploit do_deref_loc_complete; eauto.
-              exploit do_assign_loc_complete; eauto.
-              congruence.
-        -- apply not_invert_ok; simpl; intros; myinv.
-           exploit do_deref_loc_complete; eauto.           
+        exploit do_deref_loc_sound; eauto. intros [R S].
+        tagdestr; [| apply topred_ok; eapply failred_assign_mem1; eauto].
+        tagdestr; [| apply topred_ok; eapply failred_assign_mem2; eauto].
+        destruct (do_assign_loc w' ty m ofs pt bf (v,vt1) lts0) as [[[[w'' t'] m'] [v'' vt']]|] eqn:?.
+        ++ exploit do_assign_loc_sound; eauto. intros [P Q].
+           apply topred_ok; auto.
+           split. inversion P; subst; eapply red_assign_mem; eauto.
+           exists w''. eapply possible_trace_app; eauto.
+        ++ apply not_invert_ok; simpl; intros. myinv.
+           eapply do_deref_loc_complete in H1; eauto.
+           rewrite H1 in Heqo2. inv Heqo2.
+           eapply H3 in E; eauto. myinv.
+           eapply do_assign_loc_complete in H4; eauto.
            congruence.
       * (* Ltmp *)
         rewrite (is_loc_inv _ _ _ Heqo).
-        destruct (is_val a2) as [[[v2 vt2] ty2] | ] eqn:?; [| eapply incontext2_ok; eauto].
+        destruct (is_val a2) as [[[v2 vt2] ty2] | ] eqn:?; [| eapply incontext_ok; eauto].
         rewrite (is_val_inv _ _ _ Heqo0).
         destruct (type_eq ty1 ty)... subst ty1.
         destruct (te!b0) as [[v1 vt1]|] eqn:?...
@@ -1936,8 +1879,8 @@ Proof with (try (apply not_invert_ok; simpl; intro; myinv; intuition congruence;
         tagdestr_ok. apply topred_ok. split. eapply red_assign_tmp; eauto. exists w; constructor.
       * (* Lfun *)
         rewrite (is_loc_inv _ _ _ Heqo).
-        destruct (is_val a2) as [[[v2 vt2] ty2] | ] eqn:?; [| eapply incontext2_ok; eauto].
-        apply not_invert_ok; simpl; auto.
+        destruct (is_val a2) as [[[v2 vt2] ty2] | ] eqn:?; [| eapply incontext_ok; eauto].
+        apply not_invert_ok; rewrite (is_val_inv _ _ _ Heqo0); auto.
       * eapply incontext2_ok; eauto.
     + (* assignop *)
       destruct (is_loc a1) as [[[ofs pt bf| |b pt] ty1] |] eqn:?.
@@ -2017,24 +1960,23 @@ Proof with (try (apply not_invert_ok; simpl; intro; myinv; intuition congruence;
         eapply incontext2_list_ok; eauto.
       * eapply incontext2_list_ok; eauto.
     + (* builtin *)
-      admit.
-      (*destruct (is_val_list rargs) as [vtl | ] eqn:?.
+      destruct (is_val_list rargs) as [vtl | ] eqn:?.
       exploit is_val_list_all_values; eauto. intros ALLVAL.
       * (* top *)
         destruct (sem_cast_arguments vtl tyargs m) as [vargs|] eqn:?...
         destruct (do_external ef w vargs pct m) as [[[[[? ?] ?] v] m'] | ] eqn:?...
-        exploit do_ef_external_sound; eauto. intros [EC PT].
-        apply topred_ok; auto. red. split; auto. eapply red_builtin; eauto.
-        eapply sem_cast_arguments_sound; eauto.
-        exists w0; auto.
-        apply not_invert_ok; simpl; intros; myinv. specialize (H ALLVAL). myinv.
-        assert (x = vargs).
-    exploit sem_cast_arguments_complete; eauto. intros [vtl' [A B]]. congruence.
-    subst x. exploit do_ef_external_complete; eauto. congruence.
-    apply not_invert_ok; simpl; intros; myinv. specialize (H ALLVAL). myinv.
-    exploit sem_cast_arguments_complete; eauto. intros [vtl' [A B]]. congruence.
-  (* depth *)
-  eapply incontext_list_ok; eauto.*)
+        -- exploit do_ef_external_sound; eauto. intros [EC PT].
+           apply topred_ok; auto. red. split; auto. eapply red_builtin; eauto.
+           eapply sem_cast_arguments_sound; eauto.
+           exists w0; auto.
+        -- apply not_invert_ok; simpl; intros; myinv. specialize (H ALLVAL). myinv.
+           assert (x = vargs).
+           { exploit sem_cast_arguments_complete; eauto. intros [vtl' [A B]]. congruence. }
+           subst x. exploit do_ef_external_complete; eauto. congruence.
+        -- apply not_invert_ok; simpl; intros; myinv. specialize (H ALLVAL). myinv.
+           exploit sem_cast_arguments_complete; eauto. intros [vtl' [A B]]. congruence.
+      * (* depth *)
+        eapply incontext_list_ok; eauto.
 
     + (* loc *)
       split; intros. tauto. simpl; congruence.
@@ -2047,14 +1989,12 @@ Proof with (try (apply not_invert_ok; simpl; intro; myinv; intuition congruence;
       * (* depth *)
         eapply incontext_ok; eauto.
       
-  - induction al0; simpl; intros.
+  - clear step_exprlist_sound. induction al0; simpl; intros.
     + (* nil *)
       split; intros. tauto. simpl; congruence.
     + (* cons *)
       eapply incontext2_list_ok'; eauto.
-Admitted.
-
-(*Qed.*)
+Qed.
 
 Lemma step_exprlist_val_list:
   forall te m pct al, is_val_list al <> None -> step_exprlist pct al te m = nil.
@@ -2096,35 +2036,57 @@ Qed.
 Lemma lfailred_topred:
   forall pct l1 msg params te m,
     lfailred ge l1 pct msg params ->
-    step_expr LV pct l1 te m = topred (Failstopred msg params E0).
+    exists rule, step_expr LV pct l1 te m = topred (Failstopred rule msg params E0).
 Proof.
   induction 1; simpl.
-  - rewrite H. rewrite H1. rewrite H0. constructor.
-  - rewrite H. rewrite H1. rewrite H0. constructor.
+  - rewrite H. rewrite H1. rewrite H0. eexists. constructor.
+  - rewrite H. rewrite H1. rewrite H0. eexists. constructor.
 Qed.
 
 Ltac cronch :=
   match goal with
-  | [ H: ?e1 = Some _
-      |- context [match ?e1 with
-                  | Some _ => _
-                  | _ => _
-                  end] ] => rewrite H
+  | [ H: possible_trace ?w (?tr1 ++ ?tr2) ?w' |- _ ] =>
+      let w := fresh "w" in
+      let H1 := fresh "H" in
+      let H2 := fresh "H" in
+      eapply possible_trace_app_inv in H;
+      destruct H as [w [H1 H2]]
+  | [ H: ?e1 = _
+      |- match ?e1 with
+         | Some _ => _
+         | _ => _
+         end = _ ] => rewrite H
   | [ H: ?e1 = PolicySuccess _
-      |- context [match ?e1 with
-                  | PolicySuccess _ => _
-                  | PolicyFail _ _ => _
-                  end] ] => rewrite H
+      |- match ?e1 with
+         | PolicySuccess _ => _
+         | PolicyFail _ _ => _
+         end = _ ] => rewrite H
   | [ H: ?e1 = PolicyFail _ _
-      |- context [match ?e1 with
-                  | PolicySuccess _ => _
-                  | PolicyFail _ _ => _
-                  end] ] => rewrite H
+      |- match ?e1 with
+         | PolicySuccess _ => _
+         | PolicyFail _ _ => _
+         end = _ ] => rewrite H
+  | [ H: ?v = Vlong ?v' |- match ?v with
+                           | Vlong _ => _
+                           | _ => _
+                           end = _ ] =>
+      rewrite H
+  | [ |- context [type_eq ?ty ?ty] ] => rewrite dec_eq_true
+  | [ H: possible_trace ?w ?tr ?w' |- possible_trace ?w ?tr _ ] => apply H
   | [ H: deref_loc _ _ _ _ _ _ _ _ _
-      |- context [match do_deref_loc _ _ _ _ _ _ with
-                  | Some _ => _
-                  | _ => _
-                  end] ] => eapply do_deref_loc_complete in H; [rewrite H|]
+      |- match do_deref_loc _ _ _ _ _ _ with
+         | Some _ => _
+         | _ => _
+         end = _ ] => eapply do_deref_loc_complete in H; [rewrite H|]
+  | [ H: assign_loc _ _ _ _ _ _ _ _ _ _ _
+      |- match do_assign_loc _ _ _ _ _ _ _ _ with
+         | Some _ => _
+         | _ => _
+         end = _ ] => eapply do_assign_loc_complete in H; [rewrite H|]
+  | [ H: do_deref_loc _ _ _ _ _ _ = Some (_, _, ?a, _) |- _ ] =>
+      destruct a; eapply do_deref_loc_sound in H as [? ?]
+  | [ |- exists w' : world, possible_trace ?w E0 w' ] =>
+      exists w; constructor
   end.
 
 Lemma rred_topred:
@@ -2132,86 +2094,38 @@ Lemma rred_topred:
     rred ge pct1 r1 te1 m1 t pct2 r2 te2 m2 -> possible_trace w t w' ->
     exists rule, step_expr RV pct1 r1 te1 m1 = topred (Rred rule pct2 r2 te2 m2 t).
 Proof.
-  induction 1; simpl; intros.
-  (* const *)
-  - rewrite H. econstructor; eauto. 
-  (* valof_mem *)
-  - rewrite dec_eq_true.
-    eapply do_deref_loc_complete in H; eauto. rewrite H.
-    rewrite H0. rewrite H1. econstructor; eauto.
-  (* valof_fun *)
-  - rewrite dec_eq_true. econstructor; eauto.
-  (* valof_tmp*)
-  - rewrite dec_eq_true. admit. (* should !@#$ing work: rewrite H. rewrite H1. econstructor; eauto. *)
-  (* addrof_mem *)
-  - inv H. econstructor; eauto.
-  (* addrof_fun *)
-  - rewrite dec_eq_true. econstructor; eauto.
-  (* unop *)
-  - inv H0. rewrite H; econstructor; eauto.
-  (* binop *)
-  - inv H0. rewrite H; econstructor; eauto.
+  induction 1; simpl; intros; eexists; unfold atom in *; repeat cronch; try constructor; auto.
   (* cast *)
-  - inv H0. rewrite H; econstructor; eauto.
-    admit. (* TODO: cast semantics *)
-  (* seqand *)
-  - inv H0. rewrite H; econstructor; eauto.
-  - inv H0. rewrite H; econstructor; eauto.
-  (* seqor *)
-  - inv H0. rewrite H; econstructor; eauto.
-  - inv H0. rewrite H; econstructor; eauto.
-  (* condition *)
-  - inv H0. rewrite H; econstructor; eauto.
-  (* sizeof *)
-  - rewrite H. inv H0. econstructor; eauto.
-  (* alignof *)
-  - rewrite H. inv H0. econstructor; eauto.
-  (* assign_mem *)
-  - rewrite dec_eq_true. eapply possible_trace_app_inv in H4. destruct H4 as [w0 [H4 H5]].
-    rewrite H. eapply do_deref_loc_complete in H0; eauto. rewrite H0.
-    rewrite H1. rewrite H2. eapply do_assign_loc_complete in H3; eauto. rewrite H3.    
-    econstructor; eauto.
-  (* assign_tmp *)
-  - rewrite dec_eq_true. (* this !@#$ again... *)
-    admit.
-  (* assignop_mem *)
-  - rewrite dec_eq_true. eapply do_deref_loc_complete in H; eauto.
-    rewrite H. rewrite H0. rewrite H1.
-    econstructor; eauto.
-  (* assignop_tmp *)
-  - rewrite dec_eq_true. (* !@#$ *) admit.
-  (* assignop_fun *)
-  - rewrite dec_eq_true. econstructor; eauto.
-  (* postincr_mem *)
-  - rewrite dec_eq_true. eapply do_deref_loc_complete in H; eauto.
-    rewrite H. rewrite H0. rewrite H1. rewrite <- H2.
-    econstructor; eauto.
-  (* postincr_tmp *)
-  - admit. (* !@#$ *)
-  (* postincr_fun *)
-  - rewrite dec_eq_true. rewrite <- H. econstructor; eauto.
+  - destruct ty1; destruct ty; repeat cronch; eauto; congruence.
+  - subst; destruct ty1; repeat cronch; eauto; congruence.
+  - subst; destruct ty; repeat cronch; eauto; congruence.
+  - subst; repeat cronch; eauto.
+  - apply H6.
+  - rewrite H2. econstructor.
+  - destruct id; subst; econstructor.
+  - destruct id; subst; econstructor.
+  - destruct id; subst; econstructor.
   (* comma *)
-  - inv H0. rewrite dec_eq_true. econstructor; eauto.
-  (* paren *)
-  - inv H0. rewrite H. rewrite H3. econstructor; eauto.
+  - inv H. rewrite dec_eq_true. econstructor; eauto.
   (* builtin *)
   - exploit sem_cast_arguments_complete; eauto. intros [vtl [A B]].
     exploit do_ef_external_complete; eauto. intros C.
     rewrite A. rewrite B. rewrite C. econstructor; eauto.
-Admitted.
+Qed.
 
 Lemma rfailred_topred:
   forall w' pct r1 tr msg params te m,
     rfailred ge pct r1 te m tr msg params -> possible_trace w tr w' ->
-    step_expr RV pct r1 te m = topred (Failstopred msg params tr).
+    exists rule, step_expr RV pct r1 te m = topred (Failstopred rule msg params tr).
 Proof.
-  induction 1; simpl; intros; try (rewrite dec_eq_true); repeat cronch; try constructor; eauto.
-  - admit. (* !@#$ *)
-  - admit. (* !@#$ *)
-  - admit. (* !@#$ *)
-  - admit. (* !@#$ *)
+  induction 1; simpl; intros; eexists; unfold atom in *; repeat cronch; try constructor; eauto.
   - eapply sem_cast_arguments_complete in H0. destruct H0 as [vtl [P Q]]. rewrite P.
-Admitted.
+  rewrite H2. rewrite Q. rewrite H. rewrite H1. rewrite (dec_eq_true). cronch. constructor.
+  - destruct ty1; destruct ty; try congruence; repeat cronch; constructor.
+  - subst; destruct ty1; try congruence; repeat cronch; constructor.
+  - subst; destruct ty; try congruence; repeat cronch; constructor.
+  - subst; repeat cronch. constructor. eauto.
+Qed.
 
 Lemma callred_topred:
   forall pct pct' a fd args ty te m,
@@ -2388,7 +2302,7 @@ Qed.
 
 Lemma not_stuckred_imm_safe:
   forall te m a k pct,
-  (forall C, ~In (C, Stuckred) (step_expr k pct a te m)) -> imm_safe_t k a pct te m.
+    (forall C, ~In (C, Stuckred) (step_expr k pct a te m)) -> imm_safe_t k a pct te m.
 Proof.
   intros. generalize (step_expr_sound pct a k te m). intros [A B].
   destruct (step_expr k pct a te m) as [|[C rd] res] eqn:?.
@@ -2400,10 +2314,10 @@ Proof.
   exploit A. eauto with coqlib. intros [a' [k' [P [Q R]]]].
   destruct k'; destruct rd; simpl in R; intuition.
   - subst a. eapply imm_safe_t_lred; eauto.
-  - subst a. admit.
+  - subst a. eapply imm_safe_t_lfailred; eauto.
   - subst a. destruct H1 as [w' PT]. eapply imm_safe_t_rred; eauto.
   - subst. eapply imm_safe_t_callred; eauto.
-  - subst. admit.
+  - subst. eapply imm_safe_t_rfailred; eauto. (* todo: prove non-stuck implies possible trace *)
 Admitted.
 
 Lemma not_imm_safe_stuck_red:
@@ -2428,16 +2342,26 @@ Lemma imm_safe_imm_safe_t:
   forall k pct a te m,
     imm_safe ge e k a pct te m ->
     imm_safe_t k a pct te m \/
-      exists C, exists pct', exists a1, exists t, exists a1', exists te', exists m',
-        context RV k C /\ a = C a1 /\ rred ge pct a1 te m t pct' a1' te' m' /\ forall w', ~possible_trace w t w'.
+      exists C a1 tr,
+        context RV k C /\ a = C a1 /\
+          ((exists pct' a1' te' m', rred ge pct a1 te m tr pct' a1' te' m') \/
+             (exists msg params, rfailred ge pct a1 te m tr msg params))
+        /\ forall w', ~possible_trace w tr w'.
 Proof.
   intros. inv H.
   - left. apply imm_safe_t_val.
   - left. apply imm_safe_t_loc.
   - left. eapply imm_safe_t_lred; eauto.
+  - left. eapply imm_safe_t_lfailred; eauto.
   - destruct (classic (exists w', possible_trace w t0 w')) as [[w' A] | A].
     + left. eapply imm_safe_t_rred; eauto.
-    + right. exists C, PCT', e0, t0, e', te', m'; intuition.
+    + right. exists C, e0, t0; intuition.
+      left. exists PCT', e', te', m'; intuition.
+      apply A; exists w'; auto.
+  - destruct (classic (exists w', possible_trace w tr w')) as [[w' A] | A].
+    + left. eapply imm_safe_t_rfailred; eauto.
+    + right. exists C, e0, tr; intuition.
+      right. exists msg, param; intuition.
       apply A; exists w'; auto.
   - left. eapply imm_safe_t_callred; eauto.
 Qed.
@@ -2456,10 +2380,12 @@ Theorem not_imm_safe_t:
 Proof.
   intros. destruct (classic (imm_safe ge e K a pct te m)).
   - exploit imm_safe_imm_safe_t; eauto.
-    intros [A | [C1 [pct' [a1 [t [a1' [te' [m' [A [B [D E]]]]]]]]]]].
+    intros [A | [C1 [a1 [tr [A [B [[[pct' [a1' [te' [m' D]]]]|[msg [params D]]] E]]]]]]].
     + contradiction.
-    + right. red. exists t; econstructor; split; auto.
+    + right. red. exists tr; econstructor; split; auto.
       left. rewrite B. eapply step_rred with (C := fun x => C(C1 x)). eauto. eauto.
+    + right. red. exists tr; econstructor; split; auto.
+      left. rewrite B. eapply step_rfail with (C := fun x => C(C1 x)). eauto. eauto.
   - left. left. eapply step_stuck; eauto.
 Qed.
 
@@ -2467,14 +2393,15 @@ End EXPRS.
 
 (** * Transitions over states. *)
 
-Fixpoint do_alloc_variables (pct: tag) (e: env) (m: mem) (l: list (ident * type)) {struct l} : tag * env * mem :=
+Fixpoint do_alloc_variables (pct: tag) (e: env) (m: mem) (l: list (ident * type)) {struct l} :
+  tag * env * mem :=
   match l with
   | nil => (pct,e,m)
   | (id, ty) :: l' =>
-      match Mem.alloc m 0 (sizeof (snd ge) ty) with
-      | Some (m1,base1,bound1) =>
-          do_alloc_variables pct (PTree.set id (PUB (base1, bound1, def_tag)) e) m1 l'
-      | None =>
+      match Mem.alloc m 0 (sizeof (snd ge) ty), LocalT (snd ge) pct ty with
+      | Some (m',base,bound), PolicySuccess (pct', pt', lts') =>
+              do_alloc_variables pct (PTree.set id (PUB (base, bound, pt')) e) m l'
+      | _, _ =>
           (pct,e,m)
       end
   end.
@@ -2486,9 +2413,10 @@ Lemma do_alloc_variables_sound:
 Admitted.
 (*Proof.
   induction l; intros; simpl.
-  constructor.
-  destruct a as [id ty]. destruct (Mem.alloc m 0 (sizeof ge ty)) as [m1 b1] eqn:?; simpl.
-  econstructor; eauto.
+  inv H. constructor.
+  destruct a as [id ty].
+  destruct (Mem.alloc m 0 (sizeof (snd ge) ty)) as [[[m1 base1] bound1]|] eqn:?; simpl.
+  - econstructor; eauto.
 Qed.*)
 
 Lemma do_alloc_variables_complete:
@@ -2548,7 +2476,7 @@ Definition expr_final_state (f: function) (k: cont) (pct: tag) (e: env) (C_rd: (
   | Rred rule pct a te m t => TR rule t (ExprState f pct (fst C_rd a) k e te m)
   | Callred rule fd vargs ty pct' te m => TR rule E0 (Callstate fd pct' vargs (Kcall f e te pct (fst C_rd) ty k) m)
   | Stuckred => TR "step_stuck" E0 Stuckstate
-  | Failstopred msg ts tr => TR "step_failstop" tr (Failstop msg ts)
+  | Failstopred rule msg params tr => TR rule tr (Failstop msg params)
   end.
 
 Local Open Scope list_monad_scope.
@@ -2593,25 +2521,28 @@ Definition do_step (w: world) (s: Csem.state) : list transition :=
       | Some((v,vt), ty) =>
         match k with
         | Kdo k => ret "step_do_2" (State f pct Sskip k e te m )
-        | Kifthenelse s1 s2 k =>
+        | Kifthenelse s1 s2 olbl k =>
             do b <- bool_val v ty m;
-            at "step_ifthenelse_2_tfail" trule pct' <- SplitT pct vt None;
+            at "step_ifthenelse_2_tfail" trule pct' <- SplitT pct vt olbl;
             ret "step_ifthenelse_2" (State f pct' (if b then s1 else s2) k e te m)
-        | Kwhile1 x s k =>
+        | Kwhile1 x s olbl k =>
             do b <- bool_val v ty m;
+            at "step_while_tfail" trule pct' <- SplitT pct vt olbl;
             if b
-            then ret "step_while_true" (State f pct s (Kwhile2 x s k) e te m)
-            else ret "step_while_false" (State f pct Sskip k e te m)
-        | Kdowhile2 x s k =>
+            then ret "step_while_true" (State f pct' s (Kwhile2 x s olbl k) e te m)
+            else ret "step_while_false" (State f pct' Sskip k e te m)
+        | Kdowhile2 x s olbl k =>
             do b <- bool_val v ty m;
+            at "step_dowhile_tfail" trule pct' <- SplitT pct vt olbl;
             if b
-            then ret "step_dowhile_true" (State f pct (Sdowhile x s) k e te m)
-            else ret "step_dowhile_false" (State f pct Sskip k e te m)
-        | Kfor2 a2 a3 s k =>
+            then ret "step_dowhile_true" (State f pct' (Sdowhile x s olbl) k e te m)
+            else ret "step_dowhile_false" (State f pct' Sskip k e te m)
+        | Kfor2 a2 a3 s olbl k =>
             do b <- bool_val v ty m;
+            at "step_for_tfail" trule pct' <- SplitT pct vt olbl;
             if b
-            then ret "step_for_true" (State f pct s (Kfor3 a2 a3 s k) e te m)
-            else ret "step_for_false" (State f pct Sskip k e te m)
+            then ret "step_for_true" (State f pct' s (Kfor3 a2 a3 s olbl k) e te m)
+            else ret "step_for_false" (State f pct' Sskip k e te m)
         | Kreturn k =>
             do v' <- sem_cast v ty f.(fn_return) m;
             do m' <- Mem.free_list m (blocks_of_env e);
@@ -2637,33 +2568,33 @@ Definition do_step (w: world) (s: Csem.state) : list transition :=
   | State f pct Sbreak (Kseq s k) e te m =>
       ret "step_break_seq" (State f pct Sbreak k e te m)
 
-  | State f pct (Sifthenelse a s1 s2) k e te m =>
-      ret "step_ifthenelse_1" (ExprState f pct a (Kifthenelse s1 s2 k) e te m)
+  | State f pct (Sifthenelse a s1 s2 olbl) k e te m =>
+      ret "step_ifthenelse_1" (ExprState f pct a (Kifthenelse s1 s2 olbl k) e te m)
 
-  | State f pct (Swhile x s) k e te m =>
-      ret "step_while" (ExprState f pct x (Kwhile1 x s k) e te m)
-  | State f pct (Sskip|Scontinue) (Kwhile2 x s k) e te m =>
-      ret "step_skip_or_continue_while" (State f pct (Swhile x s) k e te m)
-  | State f pct Sbreak (Kwhile2 x s k) e te m =>
+  | State f pct (Swhile x s olbl) k e te m =>
+      ret "step_while" (ExprState f pct x (Kwhile1 x s olbl k) e te m)
+  | State f pct (Sskip|Scontinue) (Kwhile2 x s olbl k) e te m =>
+      ret "step_skip_or_continue_while" (State f pct (Swhile x s olbl) k e te m)
+  | State f pct Sbreak (Kwhile2 x s olbl k) e te m =>
       ret "step_break_while" (State f pct Sskip k e te m)
 
-  | State f pct (Sdowhile a s) k e te m =>
-      ret "step_dowhile" (State f pct s (Kdowhile1 a s k) e te m)
-  | State f pct (Sskip|Scontinue) (Kdowhile1 x s k) e te m =>
-      ret "step_skip_or_continue_dowhile" (ExprState f pct x (Kdowhile2 x s k) e te m)
-  | State f pct Sbreak (Kdowhile1 x s k) e te m =>
+  | State f pct (Sdowhile a s olbl) k e te m =>
+      ret "step_dowhile" (State f pct s (Kdowhile1 a s olbl k) e te m)
+  | State f pct (Sskip|Scontinue) (Kdowhile1 x s olbl k) e te m =>
+      ret "step_skip_or_continue_dowhile" (ExprState f pct x (Kdowhile2 x s olbl k) e te m)
+  | State f pct Sbreak (Kdowhile1 x s olbl k) e te m =>
       ret "step_break_dowhile" (State f pct Sskip k e te m)
 
-  | State f pct (Sfor a1 a2 a3 s) k e te m =>
+  | State f pct (Sfor a1 a2 a3 s olbl) k e te m =>
       if is_skip a1
-      then ret "step_for" (ExprState f pct a2 (Kfor2 a2 a3 s k) e te m)
-      else ret "step_for_start" (State f pct a1 (Kseq (Sfor Sskip a2 a3 s) k) e te m)
-  | State f pct (Sskip|Scontinue) (Kfor3 a2 a3 s k) e te m =>
-      ret "step_skip_or_continue_for3" (State f pct a3 (Kfor4 a2 a3 s k) e te m)
-  | State f pct Sbreak (Kfor3 a2 a3 s k) e te m =>
+      then ret "step_for" (ExprState f pct a2 (Kfor2 a2 a3 s olbl k) e te m)
+      else ret "step_for_start" (State f pct a1 (Kseq (Sfor Sskip a2 a3 s olbl) k) e te m)
+  | State f pct (Sskip|Scontinue) (Kfor3 a2 a3 s olbl k) e te m =>
+      ret "step_skip_or_continue_for3" (State f pct a3 (Kfor4 a2 a3 s olbl k) e te m)
+  | State f pct Sbreak (Kfor3 a2 a3 s olbl k) e te m =>
       ret "step_break_for3" (State f pct Sskip k e te m)
-  | State f pct Sskip (Kfor4 a2 a3 s k) e te m =>
-      ret "step_skip_for4" (State f pct (Sfor Sskip a2 a3 s) k e te m)
+  | State f pct Sskip (Kfor4 a2 a3 s olbl k) e te m =>
+      ret "step_skip_for4" (State f pct (Sfor Sskip a2 a3 s olbl) k e te m)
 
   | State f pct (Sreturn None) k e te m =>
       do m' <- Mem.free_list m (blocks_of_env e);
@@ -2779,13 +2710,13 @@ Proof with try (left; right; econstructor; eauto; fail).
       eapply do_ef_external_sound; eauto.
   (* returnstate *)
   - destruct res. destruct k; myinv...
-    + intros. left. right. admit.
-    + admit.
+    destruct res. left. inv H; inv H0.
+    right. constructor. auto.
   (* stuckstate *)
   - contradiction.
   (* failstop *)
   - contradiction.
-Admitted.
+Qed.
 
 Remark estep_not_val:
   forall f pct a k e te m t S, estep ge (ExprState f pct a k e te m) t S -> is_val a = None.
@@ -2850,24 +2781,22 @@ Proof with (unfold ret; eauto with coqlib).
       apply in_map. eauto.
     (* lfailred *)
     + unfold do_step; rewrite NOTVAL.
-      exists "step_failstop".
       exploit lfailred_topred; eauto.
       instantiate (4:=e). instantiate (3:=w). instantiate (2:=te). instantiate (1:=m).
-      intros STEP.
-      change (TR "step_failstop" E0 (Failstop msg params)) with
-        (expr_final_state f k PCT e (C, Failstopred msg params E0)).
+      intros [rule STEP]. exists rule.
+      change (TR rule E0 (Failstop msg params)) with
+        (expr_final_state f k PCT e (C, Failstopred rule msg params E0)).
       apply in_map.
       generalize (step_expr_context e w _ _ _ H1 PCT a te m). unfold reducts_incl.
       intro. replace C with (fun x => C x) by (apply extensionality; auto). apply H2.
       rewrite STEP; unfold topred; auto with coqlib.
     (* rfailred *)
     + unfold do_step; rewrite NOTVAL.
-      exists "step_failstop".
       exploit rfailred_topred; eauto.
       instantiate (1:=e).
-      intros STEP.
-      change (TR "step_failstop" t0 (Failstop msg params)) with
-        (expr_final_state f k PCT e (C, Failstopred msg params t0)).
+      intros [rule STEP]. exists rule.
+      change (TR rule t0 (Failstop msg params)) with
+        (expr_final_state f k PCT e (C, Failstopred rule msg params t0)).
       apply in_map.
       generalize (step_expr_context e w _ _ _ H1 PCT a te m). unfold reducts_incl.
       intro. replace C with (fun x => C x) by (apply extensionality; auto). apply H2.
@@ -2877,16 +2806,19 @@ Proof with (unfold ret; eauto with coqlib).
     + destruct v...
     + rewrite H0; rewrite H1...
     + rewrite H0; rewrite H1...
-    + rewrite H0...
-    + rewrite H0...
+    + rewrite H0; rewrite H1...
     + destruct H0; subst s0...
     + destruct H0; subst s0...
-    + rewrite H0...
-    + rewrite H0...
+    + rewrite H0; rewrite H1...
+    + rewrite H0; rewrite H1...
     + rewrite pred_dec_false...
-    + rewrite H0...
-    + rewrite H0...
+    + rewrite H0; rewrite H1...
+    + rewrite H0; rewrite H1...
     + destruct H0; subst x...
+    + rewrite H0; rewrite H1...
+    + rewrite H0; rewrite H1...
+    + rewrite H0; rewrite H1...
+    + rewrite H0; rewrite H1...
     + rewrite H0...
     + rewrite H0; rewrite H1...
     + rewrite H1; red in H0; destruct k; simpl; try contradiction...
@@ -2898,6 +2830,7 @@ Proof with (unfold ret; eauto with coqlib).
     + rewrite pred_dec_true; auto. rewrite (do_alloc_variables_complete _ _ _ _ _ _ _ H1).
       rewrite (sem_bind_parameters_complete _ _ _ _ _ _ H2)...
     + exploit do_ef_external_complete; eauto. intro EQ; rewrite EQ. auto with coqlib.
+    + rewrite H0...
     + rewrite H0...
 Qed.
 
